Complete TLet wand denotation proof

Denotation/theories/TLetSupport.v
@@ -4,6 +4,11 @@
 
 From Denotation Require Import Notation.
 From Denotation Require Import ContextTypeDenotation ContextTypeDenotationTactics.
+From ContextAlgebra Require Import ResourceAlgebraPullback.
+From ContextLogic Require Import FormulaSyntaxTactics.
+From CoreLang Require Import InstantiationProps.
+From Stdlib Require Import List.
+Import ListNotations.
 
 Ltac normalize_formula_fv :=
   normalize_denotation_formula_fv.
@@ -586,6 +591,327 @@ Proof.
   reflexivity.
 Qed.
 
+Lemma tm_lvars_tapp_tm_fvar e y :
+  tm_lvars (tapp_tm e (vfvar y)) = tm_lvars e ∪ {[LVFree y]}.
+Proof.
+  unfold tapp_tm, tm_lvars.
+  cbn [tm_lvars_at value_lvars_at value_shift].
+  unfold bvar_lvars_at.
+  destruct (decide (1 <= 0)); [lia|].
+  set_solver.
+Qed.
+
+Fixpoint tapp_tm_fvar_spine (e : tm) (ys : list atom) : tm :=
+  match ys with
+  | [] => e
+  | y :: ys' => tapp_tm (tapp_tm_fvar_spine e ys') (vfvar y)
+  end.
+
+Lemma fv_tm_tapp_tm_fvar_spine e ys :
+  fv_tm (tapp_tm_fvar_spine e ys) = fv_tm e ∪ list_to_set ys.
+Proof.
+  induction ys as [|y ys IH]; cbn [tapp_tm_fvar_spine].
+  - set_solver.
+  - rewrite fv_tapp_tm, IH. cbn [fv_value].
+    set_solver.
+Qed.
+
+Lemma tm_lvars_tapp_tm_fvar_spine e ys :
+  tm_lvars (tapp_tm_fvar_spine e ys) =
+  tm_lvars e ∪ lvars_of_atoms (list_to_set ys).
+Proof.
+  induction ys as [|y ys IH]; cbn [tapp_tm_fvar_spine].
+  - cbn [list_to_set]. unfold lvars_of_atoms. rewrite set_map_empty. set_solver.
+  - rewrite tm_lvars_tapp_tm_fvar, IH.
+    cbn [list_to_set].
+    unfold lvars_of_atoms.
+    rewrite set_map_union_L, set_map_singleton_L.
+    set_solver.
+Qed.
+
+Lemma fv_tm_tapp_tlete_assoc_spine e1 e2 y ys :
+  fv_tm (tapp_tm_fvar_spine
+    (tapp_tm (tlete e1 e2) (vfvar y)) ys) =
+  fv_tm (tapp_tm_fvar_spine
+    (tlete e1 (tapp_tm e2 (vfvar y))) ys).
+Proof.
+  rewrite !fv_tm_tapp_tm_fvar_spine.
+  rewrite fv_tm_tapp_tm_tlete_assoc. reflexivity.
+Qed.
+
+Lemma tm_lvars_tapp_tlete_assoc_spine e1 e2 y ys :
+  tm_lvars (tapp_tm_fvar_spine
+    (tapp_tm (tlete e1 e2) (vfvar y)) ys) =
+  tm_lvars (tapp_tm_fvar_spine
+    (tlete e1 (tapp_tm e2 (vfvar y))) ys).
+Proof.
+  rewrite !tm_lvars_tapp_tm_fvar_spine.
+  rewrite tm_lvars_tapp_tm_tlete_assoc_fvar. reflexivity.
+Qed.
+
+Lemma lc_tapp_tm_fvar_spine e ys :
+  lc_tm e ->
+  lc_tm (tapp_tm_fvar_spine e ys).
+Proof.
+  induction ys as [|y ys IH]; cbn [tapp_tm_fvar_spine]; intros Hlc.
+  - exact Hlc.
+  - apply lc_tapp_tm; [apply IH; exact Hlc | constructor].
+Qed.
+
+Lemma open_tapp_tm_fvar_spine_shift_bvar0_lc e ys y :
+  lc_tm (tapp_tm_fvar_spine e ys) ->
+  open_tm 0 (vfvar y)
+    (tapp_tm (tm_shift 0 (tapp_tm_fvar_spine e ys)) (vbvar 0)) =
+  tapp_tm_fvar_spine e (y :: ys).
+Proof.
+  intros Hlc.
+  cbn [tapp_tm_fvar_spine].
+  apply open_tapp_tm_shift_bvar0_lc. exact Hlc.
+Qed.
+
+Lemma basic_typing_tapp_tlete_assoc_spine Γ e1 e2 y ys T :
+  Γ ⊢ₑ tapp_tm_fvar_spine
+    (tlete e1 (tapp_tm e2 (vfvar y))) ys ⋮ T ->
+  Γ ⊢ₑ tapp_tm_fvar_spine
+    (tapp_tm (tlete e1 e2) (vfvar y)) ys ⋮ T.
+Proof.
+  induction ys as [|z ys IH] in T |- *; cbn [tapp_tm_fvar_spine].
+  - apply basic_typing_tapp_tm_tlete_assoc.
+  - intros Hty.
+    apply basic_typing_tapp_tm_fvar_inv in Hty as [Tx [Hfun Hz]].
+    eapply basic_typing_tapp_tm.
+    + apply IH. exact Hfun.
+    + exact Hz.
+Qed.
+
+Lemma basic_tm_has_ltype_tapp_tlete_assoc_spine
+    (Σ : lty_env) e1 e2 y ys T :
+  lc_tm (tlete e1 e2) ->
+  basic_tm_has_ltype Σ
+    (tapp_tm_fvar_spine (tlete e1 (tapp_tm e2 (vfvar y))) ys) T ->
+  basic_tm_has_ltype Σ
+    (tapp_tm_fvar_spine (tapp_tm (tlete e1 e2) (vfvar y)) ys) T.
+Proof.
+  intros Hlc [Hsub Hty].
+  split.
+  - rewrite tm_lvars_tapp_tlete_assoc_spine. exact Hsub.
+  - intros η Hfresh Hbv.
+    rewrite open_tm_env_lc.
+    + assert (Hfresh_src : open_env_fresh_for_lvars η
+        (dom Σ ∪ tm_lvars
+          (tapp_tm_fvar_spine (tlete e1 (tapp_tm e2 (vfvar y))) ys))).
+      { rewrite <- tm_lvars_tapp_tlete_assoc_spine. exact Hfresh. }
+      assert (Hbv_src :
+        lvars_bv (dom Σ ∪ tm_lvars
+          (tapp_tm_fvar_spine (tlete e1 (tapp_tm e2 (vfvar y))) ys)) ⊆
+        dom η).
+      { rewrite <- tm_lvars_tapp_tlete_assoc_spine. exact Hbv. }
+      pose proof (Hty η Hfresh_src Hbv_src) as Htyη.
+      rewrite open_tm_env_lc in Htyη by
+        (apply lc_tapp_tm_fvar_spine;
+         apply lc_tlete_tapp_tm_assoc_source; exact Hlc).
+      apply basic_typing_tapp_tlete_assoc_spine.
+      exact Htyη.
+    + apply lc_tapp_tm_fvar_spine.
+      apply lc_tapp_tm; [exact Hlc | constructor].
+Qed.
+
+Lemma expr_basic_typing_formula_tapp_tlete_assoc_spine
+    (Σ : lty_env) e1 e2 y ys T (m : WfWorldT) :
+  lc_tm (tlete e1 e2) ->
+  res_models m (expr_basic_typing_formula Σ
+    (tapp_tm_fvar_spine (tlete e1 (tapp_tm e2 (vfvar y))) ys) T) ->
+  res_models m (expr_basic_typing_formula Σ
+    (tapp_tm_fvar_spine (tapp_tm (tlete e1 e2) (vfvar y)) ys) T).
+Proof.
+  intros Hlc Hmodels.
+  apply expr_basic_typing_formula_models_iff in Hmodels as [HlcΣ [Hsub Hbasic]].
+  apply expr_basic_typing_formula_models_iff.
+  split; [exact HlcΣ|].
+  split; [exact Hsub|].
+  eapply basic_tm_has_ltype_tapp_tlete_assoc_spine; eauto.
+Qed.
+
+Lemma expr_eval_in_atom_store_tapp_tlete_assoc_spine σ e1 e2 y ys v :
+  store_closed σ ->
+  lc_tm (tlete e1 e2) ->
+  expr_eval_in_atom_store σ
+    (tapp_tm_fvar_spine (tlete e1 (tapp_tm e2 (vfvar y))) ys) v <->
+  expr_eval_in_atom_store σ
+    (tapp_tm_fvar_spine (tapp_tm (tlete e1 e2) (vfvar y)) ys) v.
+Proof.
+  intros Hclosed Hlc.
+  induction ys as [|z ys IH] in v |- *; cbn [tapp_tm_fvar_spine].
+  - apply expr_eval_in_atom_store_tapp_tm_tlete_assoc;
+      [exact Hclosed | exact Hlc | constructor].
+  - apply expr_eval_in_atom_store_tapp_tm_fun_equiv.
+    + exact Hclosed.
+    + apply lc_tapp_tm_fvar_spine.
+      apply lc_tlete_tapp_tm_assoc_source. exact Hlc.
+    + apply lc_tapp_tm_fvar_spine.
+      apply lc_tapp_tm; [exact Hlc | constructor].
+    + exact IH.
+Qed.
+
+Lemma expr_eval_in_atom_store_tapp_tlete_assoc_spine_closed_on σ e1 e2 y ys v :
+  store_closed (store_restrict σ (fv_tm (tapp_tm_fvar_spine
+    (tapp_tm (tlete e1 e2) (vfvar y)) ys))) ->
+  lc_tm (tlete e1 e2) ->
+  expr_eval_in_atom_store σ
+    (tapp_tm_fvar_spine (tlete e1 (tapp_tm e2 (vfvar y))) ys) v <->
+  expr_eval_in_atom_store σ
+    (tapp_tm_fvar_spine (tapp_tm (tlete e1 e2) (vfvar y)) ys) v.
+Proof.
+  intros Hclosed Hlc.
+  rewrite <- (expr_eval_in_atom_store_restrict_fv_exact σ
+    (tapp_tm_fvar_spine (tlete e1 (tapp_tm e2 (vfvar y))) ys) v).
+  rewrite <- (expr_eval_in_atom_store_restrict_fv_exact σ
+    (tapp_tm_fvar_spine (tapp_tm (tlete e1 e2) (vfvar y)) ys) v).
+  rewrite <- fv_tm_tapp_tlete_assoc_spine.
+  apply expr_eval_in_atom_store_tapp_tlete_assoc_spine; assumption.
+Qed.
+
+Lemma expr_total_on_atom_world_tapp_tlete_assoc_spine
+    e1 e2 y ys (m : WfWorldT) :
+  wfworld_closed_on
+    (fv_tm (tapp_tm_fvar_spine
+      (tapp_tm (tlete e1 e2) (vfvar y)) ys)) m ->
+  lc_tm (tlete e1 e2) ->
+  expr_total_on_atom_world
+    (tapp_tm_fvar_spine (tlete e1 (tapp_tm e2 (vfvar y))) ys) m ->
+  expr_total_on_atom_world
+    (tapp_tm_fvar_spine (tapp_tm (tlete e1 e2) (vfvar y)) ys) m.
+Proof.
+  intros Hclosed Hlc Htotal.
+  unfold expr_total_on_atom_world, expr_total_on in *.
+  destruct Htotal as [Hdom Hstores].
+  split.
+  - rewrite tm_lvars_tapp_tlete_assoc_spine. exact Hdom.
+  - intros τ Hτ.
+    destruct Hτ as [σ [Hσ ->]].
+    destruct (Hstores (lstore_lift_free σ)) as [v Heval].
+    { exists σ. split; [exact Hσ | reflexivity]. }
+    exists v.
+    apply (proj1 (expr_eval_in_atom_store_tapp_tlete_assoc_spine_closed_on
+      σ e1 e2 y ys v (Hclosed σ Hσ) Hlc)).
+    exact Heval.
+Qed.
+
+Lemma expr_total_formula_tapp_tlete_assoc_spine
+    e1 e2 y ys (m : WfWorldT) :
+  wfworld_closed_on
+    (fv_tm (tapp_tm_fvar_spine
+      (tapp_tm (tlete e1 e2) (vfvar y)) ys)) m ->
+  lc_tm (tlete e1 e2) ->
+  res_models m (expr_total_formula
+    (tapp_tm_fvar_spine (tlete e1 (tapp_tm e2 (vfvar y))) ys)) ->
+  res_models m (expr_total_formula
+    (tapp_tm_fvar_spine (tapp_tm (tlete e1 e2) (vfvar y)) ys)).
+Proof.
+  intros Hclosed Hlc Hmodels.
+  apply expr_total_atom_world_to_formula.
+  eapply expr_total_on_atom_world_tapp_tlete_assoc_spine; eauto.
+  apply expr_total_formula_to_atom_world. exact Hmodels.
+Qed.
+
+Lemma expr_result_at_world_tapp_tlete_assoc_spine
+    e1 e2 y ys z (m : WfWorldT) :
+  wfworld_closed_on
+    (fv_tm (tapp_tm_fvar_spine
+      (tapp_tm (tlete e1 e2) (vfvar y)) ys)) m ->
+  lc_tm (tlete e1 e2) ->
+  expr_result_at_world
+    (tapp_tm_fvar_spine (tlete e1 (tapp_tm e2 (vfvar y))) ys) z
+    (lraw_world (res_lift_free m)) ->
+  expr_result_at_world
+    (tapp_tm_fvar_spine (tapp_tm (tlete e1 e2) (vfvar y)) ys) z
+    (lraw_world (res_lift_free m)).
+Proof.
+  intros Hclosed Hlc Hres.
+  destruct Hres as [Hzfresh [Hdom Hstores]].
+  split.
+  - rewrite tm_lvars_tapp_tlete_assoc_spine. exact Hzfresh.
+  - split.
+    + rewrite tm_lvars_tapp_tlete_assoc_spine. exact Hdom.
+    + intros τ Hτ.
+      destruct Hτ as [σ [Hσ ->]].
+      specialize (Hstores (lstore_lift_free σ)
+        ltac:(exists σ; split; [exact Hσ | reflexivity])).
+      destruct Hstores as [_ [v [Hlookup Heval]]].
+      split.
+      * rewrite tm_lvars_tapp_tlete_assoc_spine. exact Hzfresh.
+      * exists v. split; [exact Hlookup |].
+        apply (proj1 (expr_eval_in_atom_store_tapp_tlete_assoc_spine_closed_on
+          σ e1 e2 y ys v (Hclosed σ Hσ) Hlc)).
+        exact Heval.
+Qed.
+
+Lemma expr_result_formula_tapp_tlete_assoc_spine
+    e1 e2 y ys z (m : WfWorldT) :
+  wfworld_closed_on
+    (fv_tm (tapp_tm_fvar_spine
+      (tapp_tm (tlete e1 e2) (vfvar y)) ys)) m ->
+  lc_tm (tlete e1 e2) ->
+  res_models m (expr_result_formula
+    (tapp_tm_fvar_spine (tlete e1 (tapp_tm e2 (vfvar y))) ys) z) ->
+  res_models m (expr_result_formula
+    (tapp_tm_fvar_spine (tapp_tm (tlete e1 e2) (vfvar y)) ys) z).
+Proof.
+  intros Hclosed Hlc Hmodels.
+  apply expr_result_atom_world_to_formula.
+  eapply expr_result_at_world_tapp_tlete_assoc_spine; eauto.
+  apply expr_result_formula_to_atom_world. exact Hmodels.
+Qed.
+
+Lemma expr_result_at_world_tapp_tlete_assoc_spine_rev
+    e1 e2 y ys z (m : WfWorldT) :
+  wfworld_closed_on
+    (fv_tm (tapp_tm_fvar_spine
+      (tapp_tm (tlete e1 e2) (vfvar y)) ys)) m ->
+  lc_tm (tlete e1 e2) ->
+  expr_result_at_world
+    (tapp_tm_fvar_spine (tapp_tm (tlete e1 e2) (vfvar y)) ys) z
+    (lraw_world (res_lift_free m)) ->
+  expr_result_at_world
+    (tapp_tm_fvar_spine (tlete e1 (tapp_tm e2 (vfvar y))) ys) z
+    (lraw_world (res_lift_free m)).
+Proof.
+  intros Hclosed Hlc Hres.
+  destruct Hres as [Hzfresh [Hdom Hstores]].
+  split.
+  - rewrite tm_lvars_tapp_tlete_assoc_spine in Hzfresh. exact Hzfresh.
+  - split.
+    + rewrite tm_lvars_tapp_tlete_assoc_spine in Hdom. exact Hdom.
+    + intros τ Hτ.
+      destruct Hτ as [σ [Hσ ->]].
+      specialize (Hstores (lstore_lift_free σ)
+        ltac:(exists σ; split; [exact Hσ | reflexivity])).
+      destruct Hstores as [_ [v [Hlookup Heval]]].
+      split.
+      * rewrite tm_lvars_tapp_tlete_assoc_spine in Hzfresh. exact Hzfresh.
+      * exists v. split; [exact Hlookup |].
+        apply (proj2 (expr_eval_in_atom_store_tapp_tlete_assoc_spine_closed_on
+          σ e1 e2 y ys v (Hclosed σ Hσ) Hlc)).
+        exact Heval.
+Qed.
+
+Lemma expr_result_formula_tapp_tlete_assoc_spine_rev
+    e1 e2 y ys z (m : WfWorldT) :
+  wfworld_closed_on
+    (fv_tm (tapp_tm_fvar_spine
+      (tapp_tm (tlete e1 e2) (vfvar y)) ys)) m ->
+  lc_tm (tlete e1 e2) ->
+  res_models m (expr_result_formula
+    (tapp_tm_fvar_spine (tapp_tm (tlete e1 e2) (vfvar y)) ys) z) ->
+  res_models m (expr_result_formula
+    (tapp_tm_fvar_spine (tlete e1 (tapp_tm e2 (vfvar y))) ys) z).
+Proof.
+  intros Hclosed Hlc Hmodels.
+  apply expr_result_atom_world_to_formula.
+  eapply expr_result_at_world_tapp_tlete_assoc_spine_rev; eauto.
+  apply expr_result_formula_to_atom_world. exact Hmodels.
+Qed.
+
 Lemma denot_ty_lvar_gas_insert_commute_tapp_open
     gas (Σ : lty_env) x y T1 Ty τ e2 (m : WfWorldT) :
   x <> y ->
@@ -734,9 +1060,36 @@ Proof.
         -- symmetry.
            replace (Σ !! LVFree z) with (Some t) by (symmetry; exact HΣz).
            apply storeA_restrict_lookup_some_2; [exact HΣz|exact Hztgt].
-        -- symmetry.
-           replace (Σ !! LVFree z) with (@None ty) by (symmetry; exact HΣz).
-           apply storeA_restrict_lookup_none_l. exact HΣz.
+	        -- symmetry.
+	           replace (Σ !! LVFree z) with (@None ty) by (symmetry; exact HΣz).
+	           apply storeA_restrict_lookup_none_l. exact HΣz.
+Qed.
+
+Lemma tlet_wand_arg_relevant_env_agree
+    (Σ : lty_env) T1 x y τx τr e1 e2 :
+  lty_env_closed Σ ->
+  x <> y ->
+  LVFree x ∉ context_ty_lvars τx ->
+  lty_env_restrict_lvars
+    (<[LVFree y := erase_ty τx]>
+      (denot_relevant_env (<[LVFree x := T1]> Σ)
+        (CTWand τx τr) (e2 ^^ x)))
+    (denot_relevant_lvars
+      (cty_open 0 y (cty_shift 0 τx)) (tret (vfvar y))) =
+  lty_env_restrict_lvars
+    (<[LVFree y := erase_ty τx]>
+      (denot_relevant_env Σ (CTWand τx τr) (tlete e1 e2)))
+    (denot_relevant_lvars
+      (cty_open 0 y (cty_shift 0 τx)) (tret (vfvar y))).
+Proof.
+  intros HΣ Hxy Hxτx.
+  change (denot_relevant_env (<[LVFree x := T1]> Σ)
+      (CTWand τx τr) (e2 ^^ x))
+    with (denot_relevant_env (<[LVFree x := T1]> Σ)
+      (CTArrow τx τr) (e2 ^^ x)).
+  change (denot_relevant_env Σ (CTWand τx τr) (tlete e1 e2))
+    with (denot_relevant_env Σ (CTArrow τx τr) (tlete e1 e2)).
+  apply tlet_arrow_arg_relevant_env_agree; assumption.
 Qed.
 
 Lemma lvars_open0_difference_subset_depth1
@@ -881,9 +1234,35 @@ Proof.
     with (D := (dom (Σsrc : gmap logic_var ty) : gset logic_var)).
   - exact Hlc.
   - exact HyΣ.
-  - destruct Hbasic as [Hvars _].
-    cbn [context_ty_lvars context_ty_lvars_at] in Hvars.
-    set_solver.
+	  - destruct Hbasic as [Hvars _].
+	    cbn [context_ty_lvars context_ty_lvars_at] in Hvars.
+	    set_solver.
+Qed.
+
+Lemma wand_body_relevant_env_agree_from_basic_context_ty
+    (Σsrc : lty_env) Ty y τx τr e_src e_body :
+  lc_lvars (dom (Σsrc : gmap logic_var ty) : gset logic_var) ->
+  LVFree y ∉ (dom (Σsrc : gmap logic_var ty) : gset logic_var) ->
+  basic_context_ty_lvars
+    (dom (Σsrc : gmap logic_var ty) : gset logic_var) (CTWand τx τr) ->
+  tm_lvars e_body ∖ {[LVFree y]} ⊆ tm_lvars e_src ->
+  lty_env_restrict_lvars
+    (<[LVFree y := Ty]>
+      (denot_relevant_env Σsrc (CTWand τx τr) e_src))
+    (denot_relevant_lvars (cty_open 0 y τr) e_body) =
+  lty_env_restrict_lvars (<[LVFree y := Ty]> Σsrc)
+    (denot_relevant_lvars (cty_open 0 y τr) e_body).
+Proof.
+  intros Hlc HyΣ Hbasic He.
+  change (denot_relevant_env Σsrc (CTWand τx τr) e_src)
+    with (denot_relevant_env Σsrc (CTArrow τx τr) e_src).
+  apply arrow_body_relevant_env_agree_from_basic_context_ty.
+  - exact Hlc.
+  - exact HyΣ.
+  - change (basic_context_ty_lvars
+      (dom (Σsrc : gmap logic_var ty) : gset logic_var) (CTArrow τx τr)).
+    exact Hbasic.
+  - exact He.
 Qed.
 
 Lemma denot_relevant_env_dom_subset_direct (Σ : lty_env) τ e :
@@ -972,144 +1351,532 @@ Proof.
     (<[LVFree y := Ty]> (∅ : gmap logic_var ty))) !! v = Some Tv).
   change (<[LVFree y := Ty]> (∅ : gmap logic_var ty))
     with ({[LVFree y := Ty]} : gmap logic_var ty).
-  rewrite storeA_union_singleton_insert_fresh by exact Hyrel.
-  exact Hlook.
+	  rewrite storeA_union_singleton_insert_fresh by exact Hyrel.
+	  exact Hlook.
 Qed.
 
-Lemma denot_ty_lvar_gas_tapp_tlete_assoc
-    gas (Σ : lty_env) τ e1 e2 y (m : WfWorldT) :
-  lc_tm (tlete e1 e2) ->
-  m ⊨ denot_ty_lvar_gas gas Σ τ
-    (tlete e1 (tapp_tm e2 (vfvar y))) ->
-  m ⊨ denot_ty_lvar_gas gas Σ τ
-    (tapp_tm (tlete e1 e2) (vfvar y)).
+Lemma basic_world_formula_wand_body_from_source_and_arg
+    (Σsrc : lty_env) Ty y τx τr e_src e_body (m : WfWorldT) :
+  lc_lvars (dom (Σsrc : gmap logic_var ty) : gset logic_var) ->
+  LVFree y ∉ (dom (Σsrc : gmap logic_var ty) : gset logic_var) ->
+  basic_context_ty_lvars
+    (dom (Σsrc : gmap logic_var ty) : gset logic_var) (CTWand τx τr) ->
+  tm_lvars e_body ∖ {[LVFree y]} ⊆ tm_lvars e_src ->
+  m ⊨ basic_world_formula (denot_relevant_env Σsrc (CTWand τx τr) e_src) ->
+  m ⊨ basic_world_formula
+    ((<[LVFree y := Ty]> (∅ : gmap logic_var ty)) : lty_env) ->
+  m ⊨ basic_world_formula
+    (denot_relevant_env (<[LVFree y := Ty]> Σsrc)
+      (cty_open 0 y τr) e_body).
 Proof.
-  (* Operational associativity for the derived application form:
-     applying the result of [let e1 in e2] to [y] is observationally the
-     same as evaluating [e1] first and then applying the opened body.  This
-     should be proved below the context-type denotation layer from the small-step
-     let decomposition/recomposition lemmas, and then lifted through the
-     recursive denotation by gas induction.
+  intros Hlc HyΣ Hbasic He Hsrc Hy.
+  change (denot_relevant_env Σsrc (CTWand τx τr) e_src)
+    with (denot_relevant_env Σsrc (CTArrow τx τr) e_src) in Hsrc.
+  eapply basic_world_formula_arrow_body_from_source_and_arg; eauto.
+Qed.
 
-     Proof plan, serving the top-level Arrow case:
+Lemma tlet_wand_arg_source_from_target
+    gas (Σ : lty_env) T1 x y τx τr e1 e2 (n : WfWorldT) :
+  lty_env_closed Σ ->
+  x <> y ->
+  LVFree x ∉ context_ty_lvars τx ->
+  y ∉ fv_cty τx ->
+  LVFree y ∉ dom
+    (denot_relevant_env Σ (CTWand τx τr) (tlete e1 e2) : lty_env) ->
+  LVFree y ∉ dom
+    (denot_relevant_env (<[LVFree x := T1]> Σ)
+      (CTWand τx τr) (e2 ^^ x) : lty_env) ->
+  n ⊨ formula_open 0 y
+    (denot_ty_lvar_gas gas
+      (typed_lty_env_bind
+        (denot_relevant_env Σ (CTWand τx τr) (tlete e1 e2))
+        (erase_ty τx))
+      (cty_shift 0 τx) (tret (vbvar 0))) ->
+  n ⊨ formula_open 0 y
+    (denot_ty_lvar_gas gas
+      (typed_lty_env_bind
+        (denot_relevant_env (<[LVFree x := T1]> Σ)
+          (CTWand τx τr) (e2 ^^ x))
+        (erase_ty τx))
+      (cty_shift 0 τx) (tret (vbvar 0))).
+Proof.
+  intros HΣ Hxy Hxτx Hyτx Hy_target_rel Hy_source_rel Harg.
+  assert (Hclosed_target_rel : lty_env_closed
+    (denot_relevant_env Σ (CTWand τx τr) (tlete e1 e2))).
+  { apply denot_relevant_env_closed. exact HΣ. }
+  assert (Hclosed_source_rel : lty_env_closed
+    (denot_relevant_env (<[LVFree x := T1]> Σ)
+      (CTWand τx τr) (e2 ^^ x))).
+  { apply denot_relevant_env_closed. apply lty_env_closed_insert_free. exact HΣ. }
+  pose proof (res_models_open_denot_ty_lvar_gas_to_open
+    y gas
+    (denot_relevant_env Σ (CTWand τx τr) (tlete e1 e2))
+    (erase_ty τx) (cty_shift 0 τx) (tret (vbvar 0)) n
+    Hy_target_rel Hclosed_target_rel
+    ltac:(cbn [fv_tm fv_value]; set_solver)
+    ltac:(rewrite cty_shift_fv; exact Hyτx)
+    Harg) as Harg_open.
+  eapply res_models_open_denot_ty_lvar_gas_from_open;
+    [ exact Hy_source_rel
+    | exact Hclosed_source_rel
+    | cbn [fv_tm fv_value]; set_solver
+    | rewrite cty_shift_fv; exact Hyτx
+    | ].
+  eapply res_models_denot_ty_lvar_gas_env_agree_on
+    with (X := denot_relevant_lvars
+      (cty_open 0 y (cty_shift 0 τx)) (tret (vfvar y))).
+  - reflexivity.
+  - symmetry.
+    apply tlet_wand_arg_relevant_env_agree; assumption.
+  - exact Harg_open.
+Qed.
 
-     1. Prove or reuse the operational equivalence already available in
-        BasicDenotation:
-        [expr_eval_in_atom_store_tapp_tm_tlete_assoc] and its FV/support
-        companions say that
-        [tlete e1 (tapp_tm e2 (vfvar y))] and
-        [tapp_tm (tlete e1 e2) (vfvar y)] have the same observable results
-        on every store, under the local closedness premise.
+Lemma tlet_wand_source_arg_fresh_x
+    gas (Σ : lty_env) T1 x y τx τr (e1 e2 : tm) :
+  lty_env_closed Σ ->
+  x <> y ->
+  LVFree x ∉ context_ty_lvars τx ->
+  x ∉ formula_fv
+    (formula_open 0 y
+      (denot_ty_lvar_gas gas
+        (typed_lty_env_bind
+          (denot_relevant_env (<[LVFree x := T1]> Σ)
+            (CTWand τx τr) (e2 ^^ x))
+          (erase_ty τx))
+        (cty_shift 0 τx) (tret (vbvar 0)))).
+Proof.
+  intros _ Hxy Hxτx Hbad.
+  pose proof (formula_open_fv_subset 0 y
+    (denot_ty_lvar_gas gas
+      (typed_lty_env_bind
+        (denot_relevant_env (<[LVFree x := T1]> Σ)
+          (CTWand τx τr) (e2 ^^ x))
+        (erase_ty τx))
+      (cty_shift 0 τx) (tret (vbvar 0)))) as Hopen.
+  pose proof (Hopen x Hbad) as Hpre_or_y.
+  apply elem_of_union in Hpre_or_y as [Hpre | Hy].
+  - pose proof (formula_fv_denot_ty_lvar_gas_subset_relevant gas
+      (typed_lty_env_bind
+        (denot_relevant_env (<[LVFree x := T1]> Σ)
+          (CTWand τx τr) (e2 ^^ x))
+        (erase_ty τx))
+      (cty_shift 0 τx) (tret (vbvar 0)) x Hpre) as Hrel.
+	    cbn [fv_tm fv_value] in Hrel.
+	    rewrite cty_shift_fv in Hrel.
+	    unfold fv_cty in Hrel.
+	    apply elem_of_union in Hrel as [Hempty | Hx_fv].
+	    + set_solver.
+	    + rewrite lvars_fv_elem in Hx_fv.
+	      contradiction.
+  - apply elem_of_singleton in Hy. congruence.
+Qed.
 
-     2. Lift that operational equivalence through the formula atoms in
-        [denot_ty_lvar_gas]:
-        - [expr_basic_typing_formula] should be transported using the same
-          basic typing derivation shape, or a small basic-typing congruence
-          for this derived application associativity.
-        - [expr_total_formula] and [expr_result_formula] should use the
-          operational equivalence wrappers from BasicDenotation.
+Lemma tlet_wand_source_body_open_for_ih
+    gas (Σ : lty_env) T1 x y τx τr e2 (w : WfWorldT) :
+  lty_env_closed Σ ->
+  x <> y ->
+  LVFree x ∉ context_ty_lvars (CTWand τx τr) ->
+  LVFree y ∉ dom
+    (denot_relevant_env (<[LVFree x := T1]> Σ)
+      (CTWand τx τr) (e2 ^^ x) : lty_env) ->
+  LVFree y ∉ dom (<[LVFree x := T1]> Σ : lty_env) ->
+  lc_tm (e2 ^^ x) ->
+  y ∉ fv_tm (tapp_tm (tm_shift 0 (e2 ^^ x)) (vbvar 0)) ->
+  y ∉ fv_cty τr ->
+  basic_context_ty_lvars
+    (dom (<[LVFree x := T1]> Σ : lty_env) : gset logic_var)
+    (CTWand τx τr) ->
+  w ⊨ formula_open 0 y
+    (denot_ty_lvar_gas gas
+      (typed_lty_env_bind
+        (denot_relevant_env (<[LVFree x := T1]> Σ)
+          (CTWand τx τr) (e2 ^^ x))
+        (erase_ty τx))
+      τr
+      (tapp_tm (tm_shift 0 (e2 ^^ x)) (vbvar 0))) ->
+  w ⊨ denot_ty_lvar_gas gas
+    (<[LVFree x := T1]> (<[LVFree y := erase_ty τx]> Σ))
+    (cty_open 0 y τr)
+    ((tapp_tm e2 (vfvar y)) ^^ x).
+Proof.
+  intros HΣ Hxy Hxfresh Hy_source_rel Hy_insert Hlc_e2x Hy_body_fv Hyτr
+    Hbasic_src_rel Hsource_body.
+  assert (Hclosed_source_rel : lty_env_closed
+    (denot_relevant_env (<[LVFree x := T1]> Σ)
+      (CTWand τx τr) (e2 ^^ x))).
+  { apply denot_relevant_env_closed. apply lty_env_closed_insert_free. exact HΣ. }
+  pose proof (res_models_open_denot_ty_lvar_gas_to_open
+    y gas
+    (denot_relevant_env (<[LVFree x := T1]> Σ)
+      (CTWand τx τr) (e2 ^^ x))
+    (erase_ty τx) τr
+    (tapp_tm (tm_shift 0 (e2 ^^ x)) (vbvar 0)) w
+    Hy_source_rel Hclosed_source_rel Hy_body_fv Hyτr
+    Hsource_body) as Hopened.
+  cbn [open_tm open_value value_shift] in Hopened.
+  assert (Hbody_full :
+    w ⊨ denot_ty_lvar_gas gas
+      (<[LVFree y := erase_ty τx]>
+        (<[LVFree x := T1]> Σ))
+      (cty_open 0 y τr)
+      (tapp_tm (e2 ^^ x) (vfvar y))).
+  {
+    eapply res_models_denot_ty_lvar_gas_env_agree_on
+      with (X := denot_relevant_lvars (cty_open 0 y τr)
+        (tapp_tm (e2 ^^ x) (vfvar y))).
+    - reflexivity.
+	    - apply wand_body_relevant_env_agree_from_basic_context_ty.
+	      + apply (proj2 (lc_lvars_no_bv _)).
+	        apply lty_env_closed_insert_free. exact HΣ.
+	      + exact Hy_insert.
+	      + exact Hbasic_src_rel.
+      + apply tm_lvars_tapp_tm_fvar_without_arg.
+    - change (w ⊨ denot_ty_lvar_gas gas
+        (<[LVFree y := erase_ty τx]>
+          (denot_relevant_env (<[LVFree x := T1]> Σ)
+            (CTWand τx τr) (e2 ^^ x)))
+        (cty_open 0 y τr)
+        (tlete (open_tm 0 (vfvar y) (tm_shift 0 (e2 ^^ x)))
+          (tapp (vbvar 0) (vfvar y)))) in Hopened.
+      rewrite open_tm_shift0_lc in Hopened by exact Hlc_e2x.
+      change (tlete (e2 ^^ x) (tapp (vbvar 0) (vfvar y)))
+        with (tapp_tm (e2 ^^ x) (vfvar y)) in Hopened.
+      exact Hopened.
+  }
+  eapply denot_ty_lvar_gas_insert_commute_tapp_open;
+    [exact Hxy | exact Hbody_full].
+Qed.
 
-     3. Induct on [gas] and destruct [τ].  The guard part is transported by
-        step 2.  Inter/Union/Sum recurse directly.  Over/Under/Arrow/Wand
-        use the fact that the recursive body formulas only inspect the same
-        FV after rewriting the term by the operational equivalence; any
-        world-transport side conditions should be discharged with the existing
-        FV upper-bound/scope helpers rather than by unfolding models.
+Lemma res_product_le_r_tlet (n m : WfWorldT)
+    (Hc : world_compat n m) :
+  m ⊑ res_product n m Hc.
+Proof.
+  destruct (res_product_comm_eq n m Hc) as [Hc' Heq].
+  rewrite Heq.
+  apply resA_le_product_l.
+Qed.
 
-     4. This lemma is used at the end of the Arrow branch of
-        [tlet_intro_denotation], after the IH has produced the denotation for
-        [tlete e1 (tapp_tm e2 (vfvar y))].  Its only job there is to change
-        the result term into the canonical Arrow result
-        [tapp_tm (tlete e1 e2) (vfvar y)]. *)
-Admitted.
-
-Lemma tlet_intro_denotation_wand_case
-    gas (Σ : lty_env) (T1 : ty) (e1 e2 : tm)
+Lemma tlet_intro_denotation_gas_zero_support
+    (Σ : lty_env) (T1 : ty) (e1 e2 : tm)
     (m mx : WfWorldT) (Fx : FiberExtensionT) (x : atom)
-    τx τr :
-  (forall (Σ : lty_env) (T1 : ty) (e1 e2 : tm)
-     (m mx : WfWorldT) (Fx : FiberExtensionT) (x : atom)
-     (τ : context_ty),
-    lty_env_closed Σ ->
-    lty_env_to_atom_env Σ ⊢ₑ e1 ⋮ T1 ->
-    lty_env_to_atom_env Σ ⊢ₑ tlete e1 e2 ⋮ erase_ty τ ->
-    expr_result_extension_witness e1 x Fx ->
-    m ⊨ expr_total_formula e1 ->
-    m ⊨ basic_world_formula (denot_relevant_env Σ τ (tlete e1 e2)) ->
-    LVFree x ∉ dom Σ ∪ context_ty_lvars τ ->
-    res_extend_by m Fx mx ->
-    mx ⊨ denot_ty_lvar_gas gas (<[LVFree x := T1]> Σ) τ (e2 ^^ x) ->
-    m ⊨ denot_ty_lvar_gas gas Σ τ (tlete e1 e2)) ->
+    (τ : context_ty) :
   lty_env_closed Σ ->
   lty_env_to_atom_env Σ ⊢ₑ e1 ⋮ T1 ->
-  lty_env_to_atom_env Σ ⊢ₑ tlete e1 e2 ⋮ erase_ty (CTWand τx τr) ->
+  lty_env_to_atom_env Σ ⊢ₑ (tlete e1 e2) ⋮ erase_ty τ ->
   expr_result_extension_witness e1 x Fx ->
   m ⊨ expr_total_formula e1 ->
-  m ⊨ basic_world_formula
-    (denot_relevant_env Σ (CTWand τx τr) (tlete e1 e2)) ->
-  LVFree x ∉ dom Σ ∪ context_ty_lvars (CTWand τx τr) ->
+  m ⊨ basic_world_formula (denot_relevant_env Σ τ (tlete e1 e2)) ->
+  LVFree x ∉ dom Σ ->
+  LVFree x ∉ context_ty_lvars τ ->
   res_extend_by m Fx mx ->
-  mx ⊨ denot_ty_lvar_gas (S gas)
-    (<[LVFree x := T1]> Σ) (CTWand τx τr) (e2 ^^ x) ->
-  m ⊨ denot_ty_lvar_gas (S gas) Σ (CTWand τx τr) (tlete e1 e2).
+  mx ⊨ denot_ty_lvar_gas 0
+    (<[LVFree x := T1]> Σ) τ (e2 ^^ x) ->
+  m ⊨ denot_ty_lvar_gas 0 Σ τ (tlete e1 e2).
 Proof.
-  (* The wand branch follows the Arrow branch's forall/extension transport,
-     but the body uses separating implication, so the commuting proof must
-     additionally transport through [res_product].  This is intentionally
-     isolated as the remaining Wand-specific proof obligation rather than
-     leaving an anonymous hole in the main [tlet] theorem.
+  intros HΣ He1 Hlet HFx Htotal Hbase_world HxΣ Hxτ Hext Hmx.
+  cbn [denot_ty_lvar_gas] in Hmx |- *.
+  repeat rewrite res_models_and_iff in Hmx |- *.
+  destruct Hmx as [[Hmx_wf [Hmx_world [Hmx_basic Hmx_total]]] _].
+  split.
+  - split.
+    + apply context_ty_wf_formula_models_iff.
+      apply basic_world_formula_models_iff in Hbase_world
+        as [Hlc_base [Hscope_base _]].
+      apply context_ty_wf_formula_models_iff in Hmx_wf
+        as [_ [_ [Hvars_mx Hshape]]].
+      split; [exact Hlc_base|].
+      split; [exact Hscope_base|].
+      split; [|exact Hshape].
+      intros v Hv.
+      assert (Hv_mx : v ∈ dom (denot_relevant_env
+        (<[LVFree x := T1]> Σ) τ (e2 ^^ x))).
+      { exact (Hvars_mx v Hv). }
+      unfold denot_relevant_env, lty_env_restrict_lvars in Hv_mx |- *.
+      change (v ∈ dom (storeA_restrict
+        ((<[LVFree x := T1]> (Σ : gmap logic_var ty)) : lty_env)
+        (denot_relevant_lvars τ (e2 ^^ x)))) in Hv_mx.
+      rewrite storeA_restrict_dom in Hv_mx.
+      apply elem_of_intersection in Hv_mx as [Hv_insert _].
+      change (v ∈ dom (storeA_restrict (Σ : gmap logic_var ty)
+        (denot_relevant_lvars τ (tlete e1 e2)))).
+      rewrite storeA_restrict_dom.
+      apply elem_of_intersection. split.
+      { change (v ∈ dom ((<[LVFree x := T1]> (Σ : gmap logic_var ty))
+          : gmap logic_var ty)) in Hv_insert.
+        rewrite dom_insert_L in Hv_insert.
+        apply elem_of_union in Hv_insert as [Hvx|HvΣ].
+        - rewrite elem_of_singleton in Hvx. subst v. contradiction.
+        - exact HvΣ. }
+      { unfold denot_relevant_lvars. set_solver. }
+    + split.
+      * exact Hbase_world.
+      * split.
+        -- eapply expr_basic_typing_formula_tlete_intro; [exact Hbase_world|].
+           apply basic_typing_lty_env_to_atom_env_denot_relevant_env.
+           exact Hlet.
+        -- eapply expr_total_formula_tlete_intro_from_result_extension
+             with (Σ := denot_relevant_env Σ τ (tlete e1 e2)); eauto.
+           ++ unfold denot_relevant_env, lty_env_restrict_lvars.
+              change (LVFree x ∉ dom
+                (storeA_restrict (Σ : gmap logic_var ty)
+                   (denot_relevant_lvars τ (tlete e1 e2)))).
+              rewrite storeA_restrict_dom. set_solver.
+           ++ apply basic_typing_lty_env_to_atom_env_denot_relevant_env.
+              exact Hlet.
+  - cbn [res_models res_models_fuel formula_measure].
+    split; [apply formula_scoped_true_iff; exact I | exact I].
+Qed.
 
-     Proof plan, mirroring the proved Arrow branch:
+Definition denot_wand_body_formula
+    (gas : nat) (Σg : lty_env) (τx τr : context_ty) (e : tm) : FormulaT :=
+  let Σx := typed_lty_env_bind Σg (erase_ty τx) in
+  FImpl (basic_world_formula (<[LVBound 0 := erase_ty τx]> ∅))
+    (FWand
+      (denot_ty_lvar_gas gas Σx
+        (cty_shift 0 τx) (tret (vbvar 0)))
+      (denot_ty_lvar_gas gas Σx τr
+        (tapp_tm (tm_shift 0 e) (vbvar 0)))).
 
-     1. Normalize the premise
-        [mx ⊨ denot_ty_lvar_gas (S gas) ... (CTWand τx τr) (e2 ^^ x)]
-        into its guard and forall/wand body with [normalize_models_ands] and
-        the existing formula-open/open-env normalizers.  The guard obligations
-        are the same shape as Arrow: context-type wf, basic world, basic
-        typing, and totality for [tlete e1 e2].
 
-     2. Use [res_models_forall_ext_transport] in the same way as Arrow to
-        align the forall witness [y] and the result extension [Fx].  The
-        basic-world premise for the freshly introduced argument should be
-        solved with the existing typed-extension/basic-world helpers, not by
-        re-proving resource typing inline.
+Lemma denot_ty_lvar_guard_wfworld_closed_on_term
+    (Σ : lty_env) τ e (m : WfWorldT) :
+  m ⊨ FAnd (context_ty_wf_formula (denot_relevant_env Σ τ e) τ)
+    (FAnd (basic_world_formula (denot_relevant_env Σ τ e))
+      (FAnd
+        (expr_basic_typing_formula (denot_relevant_env Σ τ e) e
+          (erase_ty τ))
+        (expr_total_formula e))) ->
+  wfworld_closed_on (fv_tm e) m.
+Proof.
+  intros Hguard.
+  repeat rewrite res_models_and_iff in Hguard.
+  destruct Hguard as [_ [Hworld [Hbasic _]]].
+  eapply basic_world_formula_wfworld_closed_on_atoms; [|exact Hworld].
+  unfold denot_relevant_env, denot_relevant_lvars, lty_env_restrict_lvars.
+  change (lvars_of_atoms (fv_tm e) ⊆
+    dom (storeA_restrict (Σ : gmap logic_var ty)
+      (context_ty_lvars τ ∪ tm_lvars e))).
+  rewrite storeA_restrict_dom.
+  intros v Hv.
+  unfold lvars_of_atoms in Hv.
+  apply elem_of_map in Hv as [a [-> Ha]].
+  apply elem_of_intersection. split.
+  - pose proof (expr_basic_typing_formula_basic_ltype _ _ _ _ Hbasic)
+      as [Hsub _].
+    assert (Ha_lvars : LVFree a ∈ tm_lvars e).
+    { apply lvars_fv_elem. rewrite tm_lvars_fv. exact Ha. }
+    specialize (Hsub _ Ha_lvars).
+    unfold denot_relevant_env, denot_relevant_lvars,
+      lty_env_restrict_lvars in Hsub.
+    change (LVFree a ∈ dom
+      (storeA_restrict (Σ : gmap logic_var ty)
+        (context_ty_lvars τ ∪ tm_lvars e))) in Hsub.
+    rewrite storeA_restrict_dom in Hsub.
+    apply elem_of_intersection in Hsub as [HaΣ _].
+    exact HaΣ.
+  - apply elem_of_union_r.
+    apply lvars_fv_elem. rewrite tm_lvars_fv. exact Ha.
+Qed.
 
-     3. For the wand body, open the wand hypothesis with the transported
-        argument denotation.  Compared with Arrow, the extra work is only the
-        separating-implication resource split/product:
-        transport the left resource through the argument denotation, then use
-        the recursive IH on the right/resource result world.  Any commuting
-        between [my #> Fx] and [mx #> Fy] should reuse the same extension
-        transport lemmas already used by Arrow.
+Lemma denot_ty_lvar_guard_wfworld_closed_on_term_le
+    (Σ : lty_env) τ e (m n : WfWorldT) :
+  m ⊑ n ->
+  m ⊨ FAnd (context_ty_wf_formula (denot_relevant_env Σ τ e) τ)
+    (FAnd (basic_world_formula (denot_relevant_env Σ τ e))
+      (FAnd
+        (expr_basic_typing_formula (denot_relevant_env Σ τ e) e
+          (erase_ty τ))
+        (expr_total_formula e))) ->
+  wfworld_closed_on (fv_tm e) n.
+Proof.
+  intros Hle Hguard.
+  eapply wfworld_closed_on_le.
+  - repeat rewrite res_models_and_iff in Hguard.
+    destruct Hguard as [_ [_ [_ Htotal]]].
+    pose proof (res_models_fuel_scoped _ _ _ Htotal) as Hscope.
+    unfold formula_scoped_in_world in Hscope.
+    normalize_denotation_formula_fv_in Hscope.
+    exact Hscope.
+  - exact Hle.
+  - eapply denot_ty_lvar_guard_wfworld_closed_on_term.
+    exact Hguard.
+Qed.
 
-     4. The result side should then be converted back with
-        [res_models_open_denot_ty_lvar_gas_from_open] and, if the term shape
-        is [tlete e1 (tapp_tm e2 (vfvar y))], finish with
-        [denot_ty_lvar_gas_tapp_tlete_assoc].
+Lemma denot_ty_lvar_guard_tapp_tlete_assoc
+    (Σ : lty_env) τ e1 e2 y (m : WfWorldT) :
+  lc_tm (tlete e1 e2) ->
+  m ⊨ FAnd
+    (context_ty_wf_formula
+      (denot_relevant_env Σ τ (tlete e1 (tapp_tm e2 (vfvar y)))) τ)
+    (FAnd
+      (basic_world_formula
+        (denot_relevant_env Σ τ (tlete e1 (tapp_tm e2 (vfvar y)))))
+      (FAnd
+        (expr_basic_typing_formula
+          (denot_relevant_env Σ τ (tlete e1 (tapp_tm e2 (vfvar y))))
+          (tlete e1 (tapp_tm e2 (vfvar y))) (erase_ty τ))
+        (expr_total_formula (tlete e1 (tapp_tm e2 (vfvar y)))))) ->
+  m ⊨ FAnd
+    (context_ty_wf_formula
+      (denot_relevant_env Σ τ (tapp_tm (tlete e1 e2) (vfvar y))) τ)
+    (FAnd
+      (basic_world_formula
+        (denot_relevant_env Σ τ (tapp_tm (tlete e1 e2) (vfvar y))))
+      (FAnd
+        (expr_basic_typing_formula
+          (denot_relevant_env Σ τ (tapp_tm (tlete e1 e2) (vfvar y)))
+          (tapp_tm (tlete e1 e2) (vfvar y)) (erase_ty τ))
+        (expr_total_formula (tapp_tm (tlete e1 e2) (vfvar y))))).
+Proof.
+  intros Hlc Hguard.
+  repeat rewrite res_models_and_iff in Hguard |- *.
+  destruct Hguard as [Hwf [Hworld [Hbasic Htotal]]].
+  assert (Henv :
+    denot_relevant_env Σ τ (tapp_tm (tlete e1 e2) (vfvar y)) =
+    denot_relevant_env Σ τ (tlete e1 (tapp_tm e2 (vfvar y)))).
+  {
+    unfold denot_relevant_env, lty_env_restrict_lvars, denot_relevant_lvars.
+    rewrite tm_lvars_tapp_tm_tlete_assoc_fvar. reflexivity.
+  }
+  rewrite Henv.
+  split; [exact Hwf|].
+  split; [exact Hworld|].
+  split.
+  - eapply expr_basic_typing_formula_tapp_tm_tlete_assoc; eauto.
+  - assert (Hclosed :
+      wfworld_closed_on (fv_tm (tapp_tm (tlete e1 e2) (vfvar y))) m).
+    {
+      eapply basic_world_formula_wfworld_closed_on_atoms; [|exact Hworld].
+      unfold denot_relevant_env, denot_relevant_lvars, lty_env_restrict_lvars.
+      change (lvars_of_atoms (fv_tm (tapp_tm (tlete e1 e2) (vfvar y))) ⊆
+        dom (storeA_restrict (Σ : gmap logic_var ty)
+          (context_ty_lvars τ ∪ tm_lvars (tlete e1 (tapp_tm e2 (vfvar y)))))).
+      rewrite storeA_restrict_dom.
+      intros v Hv.
+      unfold lvars_of_atoms in Hv.
+      apply elem_of_map in Hv as [a [-> Ha]].
+      apply elem_of_intersection. split.
+      - pose proof (expr_basic_typing_formula_basic_ltype _ _ _ _ Hbasic)
+          as [Hsub _].
+        assert (Ha_src :
+          LVFree a ∈ tm_lvars (tlete e1 (tapp_tm e2 (vfvar y)))).
+        {
+          rewrite <- tm_lvars_tapp_tm_tlete_assoc_fvar.
+          apply lvars_fv_elem. rewrite tm_lvars_fv. exact Ha.
+        }
+        specialize (Hsub _ Ha_src).
+        change (LVFree a ∈ dom
+          (storeA_restrict (Σ : gmap logic_var ty)
+            (context_ty_lvars τ ∪
+             tm_lvars (tlete e1 (tapp_tm e2 (vfvar y)))))) in Hsub.
+        rewrite storeA_restrict_dom in Hsub.
+        apply elem_of_intersection in Hsub as [HaΣ _].
+        exact HaΣ.
+      - apply elem_of_union_r.
+        rewrite <- tm_lvars_tapp_tm_tlete_assoc_fvar.
+        apply lvars_fv_elem. rewrite tm_lvars_fv. exact Ha.
+    }
+    eapply expr_total_formula_tapp_tm_tlete_assoc; eauto.
+Qed.
 
-     5. Keep the proof local to Wand.  Do not create broad new infrastructure
-        unless a subgoal is genuinely shared with Arrow/Over or already exists
-        one layer lower. *)
-Admitted.
+Lemma denot_ty_lvar_guard_tapp_tlete_assoc_rev
+    (Σ : lty_env) τ e1 e2 y (m : WfWorldT) :
+  lc_tm (tlete e1 e2) ->
+  m ⊨ FAnd
+    (context_ty_wf_formula
+      (denot_relevant_env Σ τ (tapp_tm (tlete e1 e2) (vfvar y))) τ)
+    (FAnd
+      (basic_world_formula
+        (denot_relevant_env Σ τ (tapp_tm (tlete e1 e2) (vfvar y))))
+      (FAnd
+        (expr_basic_typing_formula
+          (denot_relevant_env Σ τ (tapp_tm (tlete e1 e2) (vfvar y)))
+          (tapp_tm (tlete e1 e2) (vfvar y)) (erase_ty τ))
+        (expr_total_formula (tapp_tm (tlete e1 e2) (vfvar y))))) ->
+  m ⊨ FAnd
+    (context_ty_wf_formula
+      (denot_relevant_env Σ τ (tlete e1 (tapp_tm e2 (vfvar y)))) τ)
+    (FAnd
+      (basic_world_formula
+        (denot_relevant_env Σ τ (tlete e1 (tapp_tm e2 (vfvar y)))))
+      (FAnd
+        (expr_basic_typing_formula
+          (denot_relevant_env Σ τ (tlete e1 (tapp_tm e2 (vfvar y))))
+          (tlete e1 (tapp_tm e2 (vfvar y))) (erase_ty τ))
+        (expr_total_formula (tlete e1 (tapp_tm e2 (vfvar y)))))).
+Proof.
+  intros Hlc Hguard.
+  repeat rewrite res_models_and_iff in Hguard |- *.
+  destruct Hguard as [Hwf [Hworld [Hbasic Htotal]]].
+  assert (Henv :
+    denot_relevant_env Σ τ (tapp_tm (tlete e1 e2) (vfvar y)) =
+    denot_relevant_env Σ τ (tlete e1 (tapp_tm e2 (vfvar y)))).
+  {
+    unfold denot_relevant_env, lty_env_restrict_lvars, denot_relevant_lvars.
+    rewrite tm_lvars_tapp_tm_tlete_assoc_fvar. reflexivity.
+  }
+  rewrite <- Henv.
+  split; [exact Hwf|].
+  split; [exact Hworld|].
+  split.
+  - eapply expr_basic_typing_formula_tapp_tm_tlete_assoc_rev; eauto.
+  - assert (Hclosed :
+      wfworld_closed_on (fv_tm (tapp_tm (tlete e1 e2) (vfvar y))) m).
+    {
+      eapply basic_world_formula_wfworld_closed_on_atoms; [|exact Hworld].
+      unfold denot_relevant_env, denot_relevant_lvars, lty_env_restrict_lvars.
+      change (lvars_of_atoms (fv_tm (tapp_tm (tlete e1 e2) (vfvar y))) ⊆
+        dom (storeA_restrict (Σ : gmap logic_var ty)
+          (context_ty_lvars τ ∪ tm_lvars (tapp_tm (tlete e1 e2) (vfvar y))))).
+      rewrite storeA_restrict_dom.
+      intros v Hv.
+      unfold lvars_of_atoms in Hv.
+      apply elem_of_map in Hv as [a [-> Ha]].
+      apply elem_of_intersection. split.
+      - pose proof (expr_basic_typing_formula_basic_ltype _ _ _ _ Hbasic)
+          as [Hsub _].
+        assert (Ha_tgt :
+          LVFree a ∈ tm_lvars (tapp_tm (tlete e1 e2) (vfvar y))).
+        { apply lvars_fv_elem. rewrite tm_lvars_fv. exact Ha. }
+        specialize (Hsub _ Ha_tgt).
+        change (LVFree a ∈ dom
+          (storeA_restrict (Σ : gmap logic_var ty)
+            (context_ty_lvars τ ∪
+             tm_lvars (tapp_tm (tlete e1 e2) (vfvar y))))) in Hsub.
+        rewrite storeA_restrict_dom in Hsub.
+        apply elem_of_intersection in Hsub as [HaΣ _].
+        exact HaΣ.
+      - apply elem_of_union_r.
+        apply lvars_fv_elem. rewrite tm_lvars_fv. exact Ha.
+    }
+    eapply expr_total_formula_tapp_tm_tlete_assoc_rev; eauto.
+Qed.
 
-Ltac open_formula_syntax_step :=
-  rewrite ?formula_open_impl;
-  rewrite ?formula_open_fibvars;
-  rewrite ?formula_open_over;
-  rewrite ?formula_open_under;
-  rewrite ?formula_open_context_ty_wf_formula;
-  rewrite ?formula_open_expr_total_formula by solve_tlet_sidecond;
-  rewrite ?formula_open_basic_world_bind0 by solve_tlet_sidecond;
-  rewrite ?formula_open_basic_world_formula;
-  rewrite ?formula_open_expr_result_formula_shift0 by solve_tlet_sidecond;
-  rewrite ?formula_open_expr_result_formula by solve_tlet_sidecond;
-  rewrite ?lvars_open_qual_vars_difference_bound0;
-  rewrite ?type_qualifier_formula_open by solve_tlet_sidecond;
-  rewrite ?open_tapp_tm_fvar_lc_arg.
-
-Ltac normalize_open_denot_goal :=
-  idtac;
-  rewrite ?open_tapp_tm_fvar_lc_arg.
+Ltac solve_tapp_tlete_guard_assoc :=
+  match goal with
+  | Hguard : ?m ⊨ context_ty_wf_formula
+        (denot_relevant_env ?Σ ?τ (tlete ?e1 (tapp_tm ?e2 (vfvar ?y)))) ?τ
+      ∧ ?m ⊨ basic_world_formula
+          (denot_relevant_env ?Σ ?τ (tlete ?e1 (tapp_tm ?e2 (vfvar ?y))))
+        ∧ ?m ⊨ expr_basic_typing_formula
+            (denot_relevant_env ?Σ ?τ (tlete ?e1 (tapp_tm ?e2 (vfvar ?y))))
+            (tlete ?e1 (tapp_tm ?e2 (vfvar ?y))) (erase_ty ?τ)
+          ∧ ?m ⊨ expr_total_formula (tlete ?e1 (tapp_tm ?e2 (vfvar ?y)))
+    |- ?m ⊨ context_ty_wf_formula
+        (denot_relevant_env ?Σ ?τ (tapp_tm (tlete ?e1 ?e2) (vfvar ?y))) ?τ
+      ∧ ?m ⊨ basic_world_formula
+          (denot_relevant_env ?Σ ?τ (tapp_tm (tlete ?e1 ?e2) (vfvar ?y)))
+        ∧ ?m ⊨ expr_basic_typing_formula
+            (denot_relevant_env ?Σ ?τ (tapp_tm (tlete ?e1 ?e2) (vfvar ?y)))
+            (tapp_tm (tlete ?e1 ?e2) (vfvar ?y)) (erase_ty ?τ)
+          ∧ ?m ⊨ expr_total_formula (tapp_tm (tlete ?e1 ?e2) (vfvar ?y)) =>
+      let Hassoc := fresh "Hguard_assoc" in
+      pose proof (denot_ty_lvar_guard_tapp_tlete_assoc
+        Σ τ e1 e2 y m ltac:(eassumption)
+        ltac:(repeat rewrite res_models_and_iff; exact Hguard)) as Hassoc;
+      repeat rewrite res_models_and_iff in Hassoc;
+      exact Hassoc
+  end.
 
 Ltac transport_open_denot_in H :=
   lazymatch type of H with
@@ -1170,6 +1937,1647 @@ Ltac transport_open_denot_from_open_in H :=
       clear H; rename Hclosed into H
   | _ => idtac
   end.
+
+Lemma denot_ty_lvar_guard_tapp_tlete_assoc_spine
+    (Σ : lty_env) τ e1 e2 y z zs (m : WfWorldT) :
+  lc_tm (tlete e1 e2) ->
+  m ⊨ FAnd
+    (context_ty_wf_formula
+      (denot_relevant_env Σ τ
+        (tapp_tm_fvar_spine (tlete e1 (tapp_tm e2 (vfvar y))) (z :: zs))) τ)
+    (FAnd
+      (basic_world_formula
+        (denot_relevant_env Σ τ
+          (tapp_tm_fvar_spine (tlete e1 (tapp_tm e2 (vfvar y))) (z :: zs))))
+      (FAnd
+        (expr_basic_typing_formula
+          (denot_relevant_env Σ τ
+            (tapp_tm_fvar_spine (tlete e1 (tapp_tm e2 (vfvar y))) (z :: zs)))
+          (tapp_tm_fvar_spine (tlete e1 (tapp_tm e2 (vfvar y))) (z :: zs))
+          (erase_ty τ))
+        (expr_total_formula
+          (tapp_tm_fvar_spine (tlete e1 (tapp_tm e2 (vfvar y))) (z :: zs))))) ->
+  m ⊨ FAnd
+    (context_ty_wf_formula
+      (denot_relevant_env Σ τ
+        (tapp_tm_fvar_spine (tapp_tm (tlete e1 e2) (vfvar y)) (z :: zs))) τ)
+    (FAnd
+      (basic_world_formula
+        (denot_relevant_env Σ τ
+          (tapp_tm_fvar_spine (tapp_tm (tlete e1 e2) (vfvar y)) (z :: zs))))
+      (FAnd
+        (expr_basic_typing_formula
+          (denot_relevant_env Σ τ
+            (tapp_tm_fvar_spine (tapp_tm (tlete e1 e2) (vfvar y)) (z :: zs)))
+          (tapp_tm_fvar_spine (tapp_tm (tlete e1 e2) (vfvar y)) (z :: zs))
+          (erase_ty τ))
+        (expr_total_formula
+          (tapp_tm_fvar_spine (tapp_tm (tlete e1 e2) (vfvar y)) (z :: zs))))).
+Proof.
+  intros Hlc Hguard.
+  repeat rewrite res_models_and_iff in Hguard |- *.
+  destruct Hguard as [Hwf [Hworld [Hbasic Htotal]]].
+  assert (Henv :
+    denot_relevant_env Σ τ
+      (tapp_tm_fvar_spine (tapp_tm (tlete e1 e2) (vfvar y)) (z :: zs)) =
+    denot_relevant_env Σ τ
+      (tapp_tm_fvar_spine (tlete e1 (tapp_tm e2 (vfvar y))) (z :: zs))).
+  {
+    unfold denot_relevant_env, lty_env_restrict_lvars, denot_relevant_lvars.
+    rewrite tm_lvars_tapp_tlete_assoc_spine. reflexivity.
+  }
+  rewrite Henv.
+  split; [exact Hwf|].
+  split; [exact Hworld|].
+  split.
+  - eapply expr_basic_typing_formula_tapp_tlete_assoc_spine; eauto.
+  - assert (Hclosed :
+      wfworld_closed_on
+        (fv_tm (tapp_tm_fvar_spine
+          (tapp_tm (tlete e1 e2) (vfvar y)) (z :: zs))) m).
+    {
+      eapply basic_world_formula_wfworld_closed_on_atoms; [|exact Hworld].
+      unfold denot_relevant_env, denot_relevant_lvars, lty_env_restrict_lvars.
+      change (lvars_of_atoms (fv_tm (tapp_tm_fvar_spine
+          (tapp_tm (tlete e1 e2) (vfvar y)) (z :: zs))) ⊆
+        dom (storeA_restrict (Σ : gmap logic_var ty)
+          (context_ty_lvars τ ∪ tm_lvars
+            (tapp_tm_fvar_spine (tlete e1 (tapp_tm e2 (vfvar y))) (z :: zs))))).
+      rewrite storeA_restrict_dom.
+      intros v Hv.
+      unfold lvars_of_atoms in Hv.
+      apply elem_of_map in Hv as [a [-> Ha]].
+      apply elem_of_intersection. split.
+      - pose proof (expr_basic_typing_formula_basic_ltype _ _ _ _ Hbasic)
+          as [Hsub _].
+        assert (Ha_src :
+          LVFree a ∈ tm_lvars
+            (tapp_tm_fvar_spine (tlete e1 (tapp_tm e2 (vfvar y))) (z :: zs))).
+        {
+          rewrite <- tm_lvars_tapp_tlete_assoc_spine.
+          apply lvars_fv_elem. rewrite tm_lvars_fv. exact Ha.
+        }
+        specialize (Hsub _ Ha_src).
+        change (LVFree a ∈ dom
+          (storeA_restrict (Σ : gmap logic_var ty)
+            (context_ty_lvars τ ∪ tm_lvars
+              (tapp_tm_fvar_spine (tlete e1 (tapp_tm e2 (vfvar y))) (z :: zs))))) in Hsub.
+        rewrite storeA_restrict_dom in Hsub.
+        apply elem_of_intersection in Hsub as [HaΣ _].
+        exact HaΣ.
+      - apply elem_of_union_r.
+        rewrite <- tm_lvars_tapp_tlete_assoc_spine.
+        apply lvars_fv_elem. rewrite tm_lvars_fv. exact Ha.
+    }
+    eapply expr_total_formula_tapp_tlete_assoc_spine; eauto.
+Qed.
+
+Ltac solve_tapp_tlete_guard_assoc_spine :=
+  match goal with
+  | Hguard : ?m ⊨ context_ty_wf_formula
+        (denot_relevant_env ?Σ ?τ
+          (tapp_tm_fvar_spine (tlete ?e1 (tapp_tm ?e2 (vfvar ?y))) (?z :: ?zs))) ?τ
+      ∧ ?m ⊨ basic_world_formula
+          (denot_relevant_env ?Σ ?τ
+            (tapp_tm_fvar_spine (tlete ?e1 (tapp_tm ?e2 (vfvar ?y))) (?z :: ?zs)))
+        ∧ ?m ⊨ expr_basic_typing_formula
+            (denot_relevant_env ?Σ ?τ
+              (tapp_tm_fvar_spine (tlete ?e1 (tapp_tm ?e2 (vfvar ?y))) (?z :: ?zs)))
+            (tapp_tm_fvar_spine (tlete ?e1 (tapp_tm ?e2 (vfvar ?y))) (?z :: ?zs))
+            (erase_ty ?τ)
+          ∧ ?m ⊨ expr_total_formula
+              (tapp_tm_fvar_spine (tlete ?e1 (tapp_tm ?e2 (vfvar ?y))) (?z :: ?zs))
+    |- ?m ⊨ context_ty_wf_formula
+        (denot_relevant_env ?Σ ?τ
+          (tapp_tm_fvar_spine (tapp_tm (tlete ?e1 ?e2) (vfvar ?y)) (?z :: ?zs))) ?τ
+      ∧ ?m ⊨ basic_world_formula
+          (denot_relevant_env ?Σ ?τ
+            (tapp_tm_fvar_spine (tapp_tm (tlete ?e1 ?e2) (vfvar ?y)) (?z :: ?zs)))
+        ∧ ?m ⊨ expr_basic_typing_formula
+            (denot_relevant_env ?Σ ?τ
+              (tapp_tm_fvar_spine (tapp_tm (tlete ?e1 ?e2) (vfvar ?y)) (?z :: ?zs)))
+            (tapp_tm_fvar_spine (tapp_tm (tlete ?e1 ?e2) (vfvar ?y)) (?z :: ?zs))
+            (erase_ty ?τ)
+          ∧ ?m ⊨ expr_total_formula
+              (tapp_tm_fvar_spine (tapp_tm (tlete ?e1 ?e2) (vfvar ?y)) (?z :: ?zs)) =>
+      let Hassoc := fresh "Hguard_assoc_spine" in
+      pose proof (denot_ty_lvar_guard_tapp_tlete_assoc_spine
+        Σ τ e1 e2 y z zs m ltac:(eassumption)
+        ltac:(repeat rewrite res_models_and_iff; exact Hguard)) as Hassoc;
+      repeat rewrite res_models_and_iff in Hassoc;
+      exact Hassoc
+  end.
+
+Lemma denot_ty_lvar_gas_tapp_tlete_assoc_spine
+    gas (Σ : lty_env) τ e1 e2 y z zs (m : WfWorldT) :
+  lty_env_closed Σ ->
+  lc_tm (tlete e1 e2) ->
+  m ⊨ denot_ty_lvar_gas gas Σ τ
+    (tapp_tm_fvar_spine (tlete e1 (tapp_tm e2 (vfvar y))) (z :: zs)) ->
+  m ⊨ denot_ty_lvar_gas gas Σ τ
+    (tapp_tm_fvar_spine (tapp_tm (tlete e1 e2) (vfvar y)) (z :: zs)).
+Proof.
+  revert Σ τ e1 e2 y z zs m.
+  induction gas as [|gas IH]; intros Σ τ e1 e2 y z zs m HΣ Hlc Hm.
+  - cbn [denot_ty_lvar_gas] in Hm |- *.
+    repeat rewrite res_models_and_iff in Hm |- *.
+    destruct Hm as [Hguard Htrue].
+    split.
+    + solve_tapp_tlete_guard_assoc_spine.
+    + exact Htrue.
+  - destruct τ as [b φ|b φ|τ1 τ2|τ1 τ2|τ1 τ2|τx τr|τx τr];
+      cbn [denot_ty_lvar_gas] in Hm |- *;
+      repeat rewrite res_models_and_iff in Hm |- *;
+      destruct Hm as [Hguard Hbody];
+      split.
+    + solve_tapp_tlete_guard_assoc_spine.
+    + lazymatch type of Hbody with
+      | m ⊨ FForall ?φsrc => eapply (res_models_forall_map_same_fv m φsrc)
+      end.
+      * apply set_eq. intros a.
+        normalize_formula_fv.
+        rewrite !tm_shift_fv;
+        try rewrite <- fv_tm_tapp_tlete_assoc_spine;
+        try rewrite <- tm_lvars_tapp_tlete_assoc_spine;
+        tauto.
+      * pose proof (denot_ty_lvar_gas_scope_from_relevant_guard
+          (S gas) Σ (CTOver b φ)
+          (tapp_tm_fvar_spine (tapp_tm (tlete e1 e2) (vfvar y)) (z :: zs)) m
+          ltac:(repeat rewrite res_models_and_iff;
+            solve_tapp_tlete_guard_assoc_spine)) as Hscope_full.
+        cbn [denot_ty_lvar_gas] in Hscope_full.
+        eapply formula_scoped_and_r; exact Hscope_full.
+      * exists (fv_tm (tapp_tm_fvar_spine
+            (tapp_tm (tlete e1 e2) (vfvar y)) (z :: zs)) ∪
+          fv_tm (tapp_tm_fvar_spine
+            (tlete e1 (tapp_tm e2 (vfvar y))) (z :: zs)) ∪
+          qual_dom φ ∪ lvars_fv (dom Σ)).
+        intros a Ha F my HFin HFout Hext Hopen.
+        repeat rewrite formula_open_impl in Hopen.
+        repeat rewrite formula_open_impl.
+        rewrite ?formula_open_basic_world_bind0 in Hopen |- *
+          by tlet_support_solver.
+        rewrite formula_open_expr_result_formula_shift0 in Hopen.
+        2:{ apply lc_tapp_tm_fvar_spine.
+            apply lc_tlete_tapp_tm_assoc_source. exact Hlc. }
+        2:{ set_solver. }
+        rewrite formula_open_expr_result_formula_shift0.
+        2:{ apply lc_tapp_tm_fvar_spine.
+            apply lc_tapp_tm; [exact Hlc | constructor]. }
+        2:{ set_solver. }
+        pose proof (res_models_fuel_scoped _ _ _ Hopen) as Hscope_src.
+        match goal with
+        | |- my ⊨ ?G =>
+            assert (Hscope_tgt_outer : formula_scoped_in_world my G)
+        end.
+        {
+          unfold formula_scoped_in_world in *.
+          normalize_denotation_formula_fv_in Hscope_src.
+          normalize_formula_fv.
+          try rewrite fv_tm_tapp_tlete_assoc_spine.
+          exact Hscope_src.
+        }
+        eapply res_models_impl_intro; [exact Hscope_tgt_outer|].
+        intros Hbasic.
+        match goal with
+        | |- my ⊨ ?G =>
+            assert (Hscope_tgt_inner : formula_scoped_in_world my G)
+        end.
+        { eapply formula_scoped_impl_r. exact Hscope_tgt_outer. }
+        eapply res_models_impl_intro; [exact Hscope_tgt_inner|].
+        intros Hresult.
+        pose proof (res_models_impl_elim _ _ _ Hopen Hbasic) as Hinner.
+        eapply res_models_impl_elim; [exact Hinner|].
+        eapply expr_result_formula_tapp_tlete_assoc_spine_rev.
+        -- rewrite fv_tm_tapp_tlete_assoc_spine.
+           eapply denot_ty_lvar_guard_wfworld_closed_on_term_le.
+           ++ eapply res_extend_by_le; exact Hext.
+           ++ repeat rewrite res_models_and_iff. exact Hguard.
+        -- exact Hlc.
+        -- exact Hresult.
+      * exact Hbody.
+    + solve_tapp_tlete_guard_assoc_spine.
+    + lazymatch type of Hbody with
+      | m ⊨ FForall ?φsrc => eapply (res_models_forall_map_same_fv m φsrc)
+      end.
+      * apply set_eq. intros a.
+        normalize_formula_fv.
+        rewrite !tm_shift_fv;
+        try rewrite <- fv_tm_tapp_tlete_assoc_spine;
+        try rewrite <- tm_lvars_tapp_tlete_assoc_spine;
+        tauto.
+      * pose proof (denot_ty_lvar_gas_scope_from_relevant_guard
+          (S gas) Σ (CTUnder b φ)
+          (tapp_tm_fvar_spine (tapp_tm (tlete e1 e2) (vfvar y)) (z :: zs)) m
+          ltac:(repeat rewrite res_models_and_iff;
+            solve_tapp_tlete_guard_assoc_spine)) as Hscope_full.
+        cbn [denot_ty_lvar_gas] in Hscope_full.
+        eapply formula_scoped_and_r; exact Hscope_full.
+      * exists (fv_tm (tapp_tm_fvar_spine
+            (tapp_tm (tlete e1 e2) (vfvar y)) (z :: zs)) ∪
+          fv_tm (tapp_tm_fvar_spine
+            (tlete e1 (tapp_tm e2 (vfvar y))) (z :: zs)) ∪
+          qual_dom φ ∪ lvars_fv (dom Σ)).
+        intros a Ha F my HFin HFout Hext Hopen.
+        repeat rewrite formula_open_impl in Hopen.
+        repeat rewrite formula_open_impl.
+        rewrite ?formula_open_basic_world_bind0 in Hopen |- *
+          by tlet_support_solver.
+        rewrite formula_open_expr_result_formula_shift0 in Hopen.
+        2:{ apply lc_tapp_tm_fvar_spine.
+            apply lc_tlete_tapp_tm_assoc_source. exact Hlc. }
+        2:{ set_solver. }
+        rewrite formula_open_expr_result_formula_shift0.
+        2:{ apply lc_tapp_tm_fvar_spine.
+            apply lc_tapp_tm; [exact Hlc | constructor]. }
+        2:{ set_solver. }
+        pose proof (res_models_fuel_scoped _ _ _ Hopen) as Hscope_src.
+        match goal with
+        | |- my ⊨ ?G =>
+            assert (Hscope_tgt_outer : formula_scoped_in_world my G)
+        end.
+        {
+          unfold formula_scoped_in_world in *.
+          normalize_denotation_formula_fv_in Hscope_src.
+          normalize_formula_fv.
+          try rewrite fv_tm_tapp_tlete_assoc_spine.
+          exact Hscope_src.
+        }
+        eapply res_models_impl_intro; [exact Hscope_tgt_outer|].
+        intros Hbasic.
+        match goal with
+        | |- my ⊨ ?G =>
+            assert (Hscope_tgt_inner : formula_scoped_in_world my G)
+        end.
+        { eapply formula_scoped_impl_r. exact Hscope_tgt_outer. }
+        eapply res_models_impl_intro; [exact Hscope_tgt_inner|].
+        intros Hresult.
+        pose proof (res_models_impl_elim _ _ _ Hopen Hbasic) as Hinner.
+        eapply res_models_impl_elim; [exact Hinner|].
+        eapply expr_result_formula_tapp_tlete_assoc_spine_rev.
+        -- rewrite fv_tm_tapp_tlete_assoc_spine.
+           eapply denot_ty_lvar_guard_wfworld_closed_on_term_le.
+           ++ eapply res_extend_by_le; exact Hext.
+           ++ repeat rewrite res_models_and_iff. exact Hguard.
+        -- exact Hlc.
+        -- exact Hresult.
+      * exact Hbody.
+    + solve_tapp_tlete_guard_assoc_spine.
+    + repeat rewrite res_models_and_iff in Hbody |- *.
+      destruct Hbody as [H1 H2].
+      split; [eapply IH | eapply IH]; eauto.
+    + solve_tapp_tlete_guard_assoc_spine.
+    + pose proof (res_models_fuel_scoped _ _ _ Hbody) as Hscope.
+      eapply res_models_or_transport_between_worlds
+        with (m := m) (φa := denot_ty_lvar_gas gas Σ τ1
+          (tapp_tm_fvar_spine (tlete e1 (tapp_tm e2 (vfvar y))) (z :: zs)))
+          (φb := denot_ty_lvar_gas gas Σ τ2
+          (tapp_tm_fvar_spine (tlete e1 (tapp_tm e2 (vfvar y))) (z :: zs))).
+      * pose proof (denot_ty_lvar_gas_scope_from_relevant_guard
+          (S gas) Σ (CTUnion τ1 τ2)
+          (tapp_tm_fvar_spine (tapp_tm (tlete e1 e2) (vfvar y)) (z :: zs)) m
+          ltac:(repeat rewrite res_models_and_iff;
+            solve_tapp_tlete_guard_assoc_spine)) as Hscope_full.
+        cbn [denot_ty_lvar_gas] in Hscope_full.
+        eapply formula_scoped_or_l.
+        eapply formula_scoped_and_r. exact Hscope_full.
+      * pose proof (denot_ty_lvar_gas_scope_from_relevant_guard
+          (S gas) Σ (CTUnion τ1 τ2)
+          (tapp_tm_fvar_spine (tapp_tm (tlete e1 e2) (vfvar y)) (z :: zs)) m
+          ltac:(repeat rewrite res_models_and_iff;
+            solve_tapp_tlete_guard_assoc_spine)) as Hscope_full.
+        cbn [denot_ty_lvar_gas] in Hscope_full.
+        eapply formula_scoped_or_r.
+        eapply formula_scoped_and_r. exact Hscope_full.
+      * intros Hτ1. eapply IH; eauto.
+      * intros Hτ2. eapply IH; eauto.
+      * exact Hbody.
+    + solve_tapp_tlete_guard_assoc_spine.
+    + pose proof (res_models_fuel_scoped _ _ _ Hbody) as Hscope.
+      apply res_models_plus_iff in Hbody as
+        [m1 [m2 [Hdef [Hle [H1 H2]]]]].
+      * eapply res_models_plus_intro_from_models; [exact Hle| |].
+        -- eapply IH; eauto.
+        -- eapply IH; eauto.
+      * exact Hscope.
+    + solve_tapp_tlete_guard_assoc_spine.
+    + lazymatch type of Hbody with
+      | m ⊨ FForall ?φsrc => eapply (res_models_forall_full_world_map m φsrc)
+      end.
+      * pose proof (denot_ty_lvar_gas_scope_from_relevant_guard
+          (S gas) Σ (CTArrow τx τr)
+          (tapp_tm_fvar_spine (tapp_tm (tlete e1 e2) (vfvar y)) (z :: zs)) m
+          ltac:(repeat rewrite res_models_and_iff;
+            solve_tapp_tlete_guard_assoc_spine)) as Hscope_full.
+        cbn [denot_ty_lvar_gas] in Hscope_full.
+        eapply formula_scoped_and_r; exact Hscope_full.
+      * exists (fv_tm (tapp_tm_fvar_spine
+            (tapp_tm (tlete e1 e2) (vfvar y)) (z :: zs)) ∪
+          fv_tm (tapp_tm_fvar_spine
+            (tlete e1 (tapp_tm e2 (vfvar y))) (z :: zs)) ∪
+          fv_cty τx ∪ fv_cty τr ∪ lvars_fv (dom Σ)).
+        intros a Ha my Hdom Hrestrict Hopen.
+        pose proof (denot_ty_lvar_gas_scope_from_relevant_guard
+          (S gas) Σ (CTArrow τx τr)
+          (tapp_tm_fvar_spine (tapp_tm (tlete e1 e2) (vfvar y)) (z :: zs)) m
+          ltac:(repeat rewrite res_models_and_iff;
+            solve_tapp_tlete_guard_assoc_spine)) as Hscope_full_my.
+        cbn [denot_ty_lvar_gas] in Hscope_full_my.
+        pose proof (formula_scoped_and_r _ _ _ Hscope_full_my)
+          as Htarget_forall_scope.
+        match goal with
+        | |- my ⊨ ?G =>
+            assert (Hopened_scope_my : formula_scoped_in_world my G)
+        end.
+        {
+          eapply formula_scoped_open_from_fv.
+          unfold formula_scoped_in_world in Htarget_forall_scope.
+          rewrite Hdom.
+          set_solver.
+        }
+        repeat rewrite formula_open_impl in Hopen.
+        repeat rewrite formula_open_impl.
+        repeat rewrite formula_open_impl in Hopened_scope_my.
+        rewrite ?formula_open_basic_world_bind0 in Hopen |- *
+          by tlet_support_solver.
+        rewrite ?formula_open_basic_world_bind0 in Hopened_scope_my
+          by tlet_support_solver.
+        eapply res_models_impl_intro; [exact Hopened_scope_my|].
+        intros Hbasic.
+        pose proof (formula_scoped_impl_r _ _ _ Hopened_scope_my)
+          as Hscope_tgt_inner.
+        eapply res_models_impl_intro; [exact Hscope_tgt_inner|].
+        intros Harg.
+        assert (Henv_arrow :
+          denot_relevant_env Σ (CTArrow τx τr)
+            (tapp_tm_fvar_spine (tapp_tm (tlete e1 e2) (vfvar y)) (z :: zs)) =
+          denot_relevant_env Σ (CTArrow τx τr)
+            (tapp_tm_fvar_spine (tlete e1 (tapp_tm e2 (vfvar y))) (z :: zs))).
+        {
+          unfold denot_relevant_env, denot_relevant_lvars,
+            lty_env_restrict_lvars.
+          rewrite tm_lvars_tapp_tlete_assoc_spine. reflexivity.
+        }
+        rewrite Henv_arrow in Harg.
+        pose proof (res_models_impl_elim _ _ _ Hopen Hbasic) as Hinner.
+        pose proof (res_models_impl_elim _ _ _ Hinner Harg) as Hres.
+        pose proof (res_models_open_denot_ty_lvar_gas_to_open
+          a gas
+          (denot_relevant_env Σ (CTArrow τx τr)
+            (tapp_tm_fvar_spine (tlete e1 (tapp_tm e2 (vfvar y))) (z :: zs)))
+          (erase_ty τx) τr
+          (tapp_tm
+            (tm_shift 0
+              (tapp_tm_fvar_spine (tlete e1 (tapp_tm e2 (vfvar y))) (z :: zs)))
+            (vbvar 0))
+          my
+          ltac:(unfold denot_relevant_env, lty_env_restrict_lvars;
+            change (LVFree a ∉ dom (storeA_restrict (Σ : gmap logic_var ty)
+              (denot_relevant_lvars (CTArrow τx τr)
+                (tapp_tm_fvar_spine
+                  (tlete e1 (tapp_tm e2 (vfvar y))) (z :: zs)))));
+            rewrite storeA_restrict_dom;
+            intros Hadom; apply elem_of_intersection in Hadom as [HaΣ _];
+            apply Ha; repeat (apply elem_of_union_r);
+            apply lvars_fv_elem; exact HaΣ)
+          ltac:(apply denot_relevant_env_closed; exact HΣ)
+          ltac:(rewrite fv_tapp_tm, tm_shift_fv; cbn [fv_value]; set_solver)
+          ltac:(set_solver)
+          Hres) as Hres_opened.
+        clear Hres. rename Hres_opened into Hres.
+        rewrite open_tapp_tm_fvar_spine_shift_bvar0_lc in Hres
+          by (apply lc_tapp_tm_fvar_spine;
+              apply lc_tlete_tapp_tm_assoc_source; exact Hlc).
+        eapply IH in Hres.
+        3:{ exact Hlc. }
+        2:{
+          apply lty_env_closed_insert_free.
+          apply denot_relevant_env_closed. exact HΣ.
+        }
+        rewrite <- Henv_arrow in Hres.
+        replace (tapp_tm_fvar_spine
+            (tapp_tm (tlete e1 e2) (vfvar y)) (a :: z :: zs))
+          with (open_tm 0 (vfvar a)
+            (tapp_tm
+              (tm_shift 0
+                (tapp_tm_fvar_spine
+                  (tapp_tm (tlete e1 e2) (vfvar y)) (z :: zs)))
+              (vbvar 0))) in Hres by
+          (rewrite open_tapp_tm_fvar_spine_shift_bvar0_lc by
+            (apply lc_tapp_tm_fvar_spine;
+             apply lc_tapp_tm; [exact Hlc | constructor]);
+           reflexivity).
+        pose proof (res_models_open_denot_ty_lvar_gas_from_open
+          a gas
+          (denot_relevant_env Σ (CTArrow τx τr)
+            (tapp_tm_fvar_spine (tapp_tm (tlete e1 e2) (vfvar y)) (z :: zs)))
+          (erase_ty τx) τr
+          (tapp_tm
+            (tm_shift 0
+              (tapp_tm_fvar_spine
+                (tapp_tm (tlete e1 e2) (vfvar y)) (z :: zs)))
+            (vbvar 0))
+          my
+          ltac:(unfold denot_relevant_env, lty_env_restrict_lvars;
+            change (LVFree a ∉ dom (storeA_restrict (Σ : gmap logic_var ty)
+              (denot_relevant_lvars (CTArrow τx τr)
+                (tapp_tm_fvar_spine
+                  (tapp_tm (tlete e1 e2) (vfvar y)) (z :: zs)))));
+            rewrite storeA_restrict_dom;
+            intros Hadom; apply elem_of_intersection in Hadom as [HaΣ _];
+            apply Ha; repeat (apply elem_of_union_r);
+            apply lvars_fv_elem; exact HaΣ)
+          ltac:(apply denot_relevant_env_closed; exact HΣ)
+          ltac:(rewrite fv_tapp_tm, tm_shift_fv; cbn [fv_value]; set_solver)
+          ltac:(set_solver)
+          Hres) as Hres_formula.
+        clear Hres. rename Hres_formula into Hres.
+        exact Hres.
+      * exact Hbody.
+    + solve_tapp_tlete_guard_assoc_spine.
+    + lazymatch type of Hbody with
+      | m ⊨ FForall ?φsrc => eapply (res_models_forall_full_world_map m φsrc)
+      end.
+      * pose proof (denot_ty_lvar_gas_scope_from_relevant_guard
+          (S gas) Σ (CTWand τx τr)
+          (tapp_tm_fvar_spine (tapp_tm (tlete e1 e2) (vfvar y)) (z :: zs)) m
+          ltac:(repeat rewrite res_models_and_iff;
+            solve_tapp_tlete_guard_assoc_spine)) as Hscope_full.
+        cbn [denot_ty_lvar_gas] in Hscope_full.
+        eapply formula_scoped_and_r; exact Hscope_full.
+      * exists (fv_tm (tapp_tm_fvar_spine
+            (tapp_tm (tlete e1 e2) (vfvar y)) (z :: zs)) ∪
+          fv_tm (tapp_tm_fvar_spine
+            (tlete e1 (tapp_tm e2 (vfvar y))) (z :: zs)) ∪
+          fv_cty τx ∪ fv_cty τr ∪ lvars_fv (dom Σ)).
+        intros a Ha my Hdom Hrestrict Hopen.
+        repeat rewrite formula_open_impl in Hopen.
+        repeat rewrite formula_open_impl.
+        rewrite ?formula_open_basic_world_bind0 in Hopen |- *
+          by tlet_support_solver.
+        rewrite !formula_open_wand in Hopen |- *.
+        pose proof (denot_ty_lvar_gas_scope_from_relevant_guard
+          (S gas) Σ (CTWand τx τr)
+          (tapp_tm_fvar_spine (tapp_tm (tlete e1 e2) (vfvar y)) (z :: zs)) m
+          ltac:(repeat rewrite res_models_and_iff;
+            solve_tapp_tlete_guard_assoc_spine)) as Hscope_full_my.
+        cbn [denot_ty_lvar_gas] in Hscope_full_my.
+        pose proof (formula_scoped_and_r _ _ _ Hscope_full_my)
+          as Htarget_forall_scope.
+        match goal with
+        | |- my ⊨ ?G =>
+            assert (Hscope_tgt_outer : formula_scoped_in_world my G)
+        end.
+        {
+          change (formula_scoped_in_world my
+            (formula_open 0 a
+              (FImpl (basic_world_formula (<[LVBound 0 := erase_ty τx]> ∅))
+                (FWand
+                  (denot_ty_lvar_gas gas
+                    (typed_lty_env_bind
+                      (denot_relevant_env Σ (CTWand τx τr)
+                        (tapp_tm_fvar_spine
+                          (tapp_tm (tlete e1 e2) (vfvar y)) (z :: zs)))
+                      (erase_ty τx))
+                    (cty_shift 0 τx) (tret (vbvar 0)))
+                  (denot_ty_lvar_gas gas
+                    (typed_lty_env_bind
+                      (denot_relevant_env Σ (CTWand τx τr)
+                        (tapp_tm_fvar_spine
+                          (tapp_tm (tlete e1 e2) (vfvar y)) (z :: zs)))
+                      (erase_ty τx))
+                    τr
+                    (tapp_tm
+                      (tm_shift 0
+                        (tapp_tm_fvar_spine
+                          (tapp_tm (tlete e1 e2) (vfvar y)) (z :: zs)))
+                      (vbvar 0))))))).
+          eapply formula_scoped_open_from_fv.
+          unfold formula_scoped_in_world in Htarget_forall_scope.
+          formula_fv_syntax_norm_in Htarget_forall_scope.
+          formula_fv_syntax_norm.
+          rewrite Hdom.
+          set_solver.
+        }
+        eapply res_models_impl_intro; [exact Hscope_tgt_outer|].
+        intros Hbasic.
+        pose proof (res_models_impl_elim _ _ _ Hopen Hbasic) as Hwand.
+        pose proof (res_models_fuel_scoped _ _ _ Hwand) as Hscope_src_wand.
+        pose proof (proj1 (res_models_wand_iff my _ _ Hscope_src_wand) Hwand)
+          as Hwand_elim.
+        clear Hwand. rename Hwand_elim into Hwand.
+        pose proof (formula_scoped_impl_r _ _ _ Hscope_tgt_outer)
+             as Hscope_tgt_wand.
+        apply (proj2 (res_models_wand_iff _ _ _ Hscope_tgt_wand)).
+        intros n1 Hc Harg.
+        assert (Henv_wand :
+          denot_relevant_env Σ (CTWand τx τr)
+            (tapp_tm_fvar_spine (tapp_tm (tlete e1 e2) (vfvar y)) (z :: zs)) =
+          denot_relevant_env Σ (CTWand τx τr)
+            (tapp_tm_fvar_spine (tlete e1 (tapp_tm e2 (vfvar y))) (z :: zs))).
+        {
+          unfold denot_relevant_env, denot_relevant_lvars,
+            lty_env_restrict_lvars.
+          rewrite tm_lvars_tapp_tlete_assoc_spine. reflexivity.
+        }
+        rewrite Henv_wand in Harg.
+        pose proof (Hwand n1 Hc Harg) as Hres.
+        pose proof (res_models_open_denot_ty_lvar_gas_to_open
+          a gas
+          (denot_relevant_env Σ (CTWand τx τr)
+            (tapp_tm_fvar_spine (tlete e1 (tapp_tm e2 (vfvar y))) (z :: zs)))
+          (erase_ty τx) τr
+          (tapp_tm
+            (tm_shift 0
+              (tapp_tm_fvar_spine (tlete e1 (tapp_tm e2 (vfvar y))) (z :: zs)))
+            (vbvar 0))
+          (res_product n1 my Hc)
+          ltac:(unfold denot_relevant_env, lty_env_restrict_lvars;
+            change (LVFree a ∉ dom (storeA_restrict (Σ : gmap logic_var ty)
+              (denot_relevant_lvars (CTWand τx τr)
+                (tapp_tm_fvar_spine
+                  (tlete e1 (tapp_tm e2 (vfvar y))) (z :: zs)))));
+            rewrite storeA_restrict_dom;
+            intros Hadom; apply elem_of_intersection in Hadom as [HaΣ _];
+            apply Ha; repeat (apply elem_of_union_r);
+            apply lvars_fv_elem; exact HaΣ)
+          ltac:(apply denot_relevant_env_closed; exact HΣ)
+          ltac:(rewrite fv_tapp_tm, tm_shift_fv; cbn [fv_value]; set_solver)
+          ltac:(set_solver)
+          Hres) as Hres_opened.
+        clear Hres. rename Hres_opened into Hres.
+        rewrite open_tapp_tm_fvar_spine_shift_bvar0_lc in Hres
+          by (apply lc_tapp_tm_fvar_spine;
+              apply lc_tlete_tapp_tm_assoc_source; exact Hlc).
+        eapply IH in Hres.
+        3:{ exact Hlc. }
+        2:{
+          apply lty_env_closed_insert_free.
+          apply denot_relevant_env_closed. exact HΣ.
+        }
+        rewrite <- Henv_wand in Hres.
+        replace (tapp_tm_fvar_spine
+            (tapp_tm (tlete e1 e2) (vfvar y)) (a :: z :: zs))
+          with (open_tm 0 (vfvar a)
+            (tapp_tm
+              (tm_shift 0
+                (tapp_tm_fvar_spine
+                  (tapp_tm (tlete e1 e2) (vfvar y)) (z :: zs)))
+              (vbvar 0))) in Hres by
+          (rewrite open_tapp_tm_fvar_spine_shift_bvar0_lc by
+            (apply lc_tapp_tm_fvar_spine;
+             apply lc_tapp_tm; [exact Hlc | constructor]);
+           reflexivity).
+        pose proof (res_models_open_denot_ty_lvar_gas_from_open
+          a gas
+          (denot_relevant_env Σ (CTWand τx τr)
+            (tapp_tm_fvar_spine (tapp_tm (tlete e1 e2) (vfvar y)) (z :: zs)))
+          (erase_ty τx) τr
+          (tapp_tm
+            (tm_shift 0
+              (tapp_tm_fvar_spine
+                (tapp_tm (tlete e1 e2) (vfvar y)) (z :: zs)))
+            (vbvar 0))
+          (res_product n1 my Hc)
+          ltac:(unfold denot_relevant_env, lty_env_restrict_lvars;
+            change (LVFree a ∉ dom (storeA_restrict (Σ : gmap logic_var ty)
+              (denot_relevant_lvars (CTWand τx τr)
+                (tapp_tm_fvar_spine
+                  (tapp_tm (tlete e1 e2) (vfvar y)) (z :: zs)))));
+            rewrite storeA_restrict_dom;
+            intros Hadom; apply elem_of_intersection in Hadom as [HaΣ _];
+            apply Ha; repeat (apply elem_of_union_r);
+            apply lvars_fv_elem; exact HaΣ)
+          ltac:(apply denot_relevant_env_closed; exact HΣ)
+          ltac:(rewrite fv_tapp_tm, tm_shift_fv; cbn [fv_value]; set_solver)
+          ltac:(set_solver)
+          Hres) as Hres_formula.
+        clear Hres. rename Hres_formula into Hres.
+        exact Hres.
+      * exact Hbody.
+Qed.
+
+Lemma denot_ty_lvar_gas_tapp_tlete_assoc_under_tapp
+    gas (Σ : lty_env) τ e1 e2 y z (m : WfWorldT) :
+  lty_env_closed Σ ->
+  lc_tm (tlete e1 e2) ->
+  m ⊨ denot_ty_lvar_gas gas Σ τ
+    (tapp_tm (tlete e1 (tapp_tm e2 (vfvar y))) (vfvar z)) ->
+  m ⊨ denot_ty_lvar_gas gas Σ τ
+    (tapp_tm (tapp_tm (tlete e1 e2) (vfvar y)) (vfvar z)).
+Proof.
+  intros HΣ Hlc Hm.
+  change (tapp_tm (tlete e1 (tapp_tm e2 (vfvar y))) (vfvar z))
+    with (tapp_tm_fvar_spine (tlete e1 (tapp_tm e2 (vfvar y))) [z]) in Hm.
+  change (tapp_tm (tapp_tm (tlete e1 e2) (vfvar y)) (vfvar z))
+    with (tapp_tm_fvar_spine (tapp_tm (tlete e1 e2) (vfvar y)) [z]).
+  eapply denot_ty_lvar_gas_tapp_tlete_assoc_spine; eauto.
+Qed.
+
+Lemma denot_ty_lvar_gas_tapp_tlete_assoc
+    gas (Σ : lty_env) τ e1 e2 y (m : WfWorldT) :
+  lty_env_closed Σ ->
+  lc_tm (tlete e1 e2) ->
+  m ⊨ denot_ty_lvar_gas gas Σ τ
+    (tlete e1 (tapp_tm e2 (vfvar y))) ->
+  m ⊨ denot_ty_lvar_gas gas Σ τ
+    (tapp_tm (tlete e1 e2) (vfvar y)).
+Proof.
+  revert Σ τ e1 e2 y m.
+  induction gas as [|gas IH]; intros Σ τ e1 e2 y m HΣ Hlc Hm.
+  - cbn [denot_ty_lvar_gas] in Hm |- *.
+    repeat rewrite res_models_and_iff in Hm |- *.
+    destruct Hm as [Hguard Htrue].
+    split.
+    + solve_tapp_tlete_guard_assoc.
+    + exact Htrue.
+  - destruct τ as [b φ|b φ|τ1 τ2|τ1 τ2|τ1 τ2|τx τr|τx τr];
+      cbn [denot_ty_lvar_gas] in Hm |- *;
+      repeat rewrite res_models_and_iff in Hm |- *;
+      destruct Hm as [Hguard Hbody];
+      split.
+    + solve_tapp_tlete_guard_assoc.
+    + lazymatch type of Hbody with
+      | m ⊨ FForall ?φsrc => eapply (res_models_forall_map_same_fv m φsrc)
+      end.
+      * apply set_eq. intros a.
+        normalize_formula_fv.
+        rewrite !tm_shift_fv;
+        try rewrite <- fv_tm_tapp_tm_tlete_assoc;
+        try rewrite <- tm_lvars_tapp_tm_tlete_assoc_fvar;
+        tauto.
+      * pose proof (denot_ty_lvar_gas_scope_from_relevant_guard
+          (S gas) Σ (CTOver b φ)
+          (tapp_tm (tlete e1 e2) (vfvar y)) m
+          ltac:(repeat rewrite res_models_and_iff;
+            solve_tapp_tlete_guard_assoc)) as Hscope_full.
+        cbn [denot_ty_lvar_gas] in Hscope_full.
+        eapply formula_scoped_and_r; exact Hscope_full.
+      * exists (fv_tm (tapp_tm (tlete e1 e2) (vfvar y)) ∪
+          fv_tm (tlete e1 (tapp_tm e2 (vfvar y))) ∪
+          qual_dom φ ∪ lvars_fv (dom Σ)).
+        intros z Hz F my HFin HFout Hext Hopen.
+        repeat rewrite formula_open_impl in Hopen.
+        repeat rewrite formula_open_impl.
+        rewrite ?formula_open_basic_world_bind0 in Hopen |- *
+          by tlet_support_solver.
+        rewrite formula_open_expr_result_formula_shift0 in Hopen.
+        2:{ apply lc_tlete_tapp_tm_assoc_source. exact Hlc. }
+        2:{ set_solver. }
+        rewrite formula_open_expr_result_formula_shift0.
+        2:{ apply lc_tapp_tm; [exact Hlc | constructor]. }
+        2:{ set_solver. }
+        pose proof (res_models_fuel_scoped _ _ _ Hopen) as Hscope_src.
+        match goal with
+        | |- my ⊨ ?G =>
+            assert (Hscope_tgt_outer : formula_scoped_in_world my G)
+        end.
+        {
+          unfold formula_scoped_in_world in *.
+          normalize_denotation_formula_fv_in Hscope_src.
+          normalize_formula_fv.
+          try rewrite fv_tm_tapp_tm_tlete_assoc.
+          exact Hscope_src.
+        }
+        eapply res_models_impl_intro; [exact Hscope_tgt_outer|].
+        intros Hbasic.
+        match goal with
+        | |- my ⊨ ?G =>
+            assert (Hscope_tgt_inner : formula_scoped_in_world my G)
+        end.
+        { eapply formula_scoped_impl_r. exact Hscope_tgt_outer. }
+        eapply res_models_impl_intro; [exact Hscope_tgt_inner|].
+        intros Hresult.
+        pose proof (res_models_impl_elim _ _ _ Hopen Hbasic) as Hinner.
+        eapply res_models_impl_elim; [exact Hinner|].
+        eapply expr_result_formula_tapp_tm_tlete_assoc_rev.
+        -- rewrite fv_tm_tapp_tm_tlete_assoc.
+           eapply denot_ty_lvar_guard_wfworld_closed_on_term_le.
+           ++ eapply res_extend_by_le; exact Hext.
+           ++ repeat rewrite res_models_and_iff. exact Hguard.
+        -- exact Hlc.
+        -- exact Hresult.
+      * exact Hbody.
+    + solve_tapp_tlete_guard_assoc.
+    + lazymatch type of Hbody with
+      | m ⊨ FForall ?φsrc => eapply (res_models_forall_map_same_fv m φsrc)
+      end.
+      * apply set_eq. intros a.
+        normalize_formula_fv.
+        rewrite !tm_shift_fv;
+        try rewrite <- fv_tm_tapp_tm_tlete_assoc;
+        try rewrite <- tm_lvars_tapp_tm_tlete_assoc_fvar;
+        tauto.
+      * pose proof (denot_ty_lvar_gas_scope_from_relevant_guard
+          (S gas) Σ (CTUnder b φ)
+          (tapp_tm (tlete e1 e2) (vfvar y)) m
+          ltac:(repeat rewrite res_models_and_iff;
+            solve_tapp_tlete_guard_assoc)) as Hscope_full.
+        cbn [denot_ty_lvar_gas] in Hscope_full.
+        eapply formula_scoped_and_r; exact Hscope_full.
+      * exists (fv_tm (tapp_tm (tlete e1 e2) (vfvar y)) ∪
+          fv_tm (tlete e1 (tapp_tm e2 (vfvar y))) ∪
+          qual_dom φ ∪ lvars_fv (dom Σ)).
+        intros z Hz F my HFin HFout Hext Hopen.
+        repeat rewrite formula_open_impl in Hopen.
+        repeat rewrite formula_open_impl.
+        rewrite ?formula_open_basic_world_bind0 in Hopen |- *
+          by tlet_support_solver.
+        rewrite formula_open_expr_result_formula_shift0 in Hopen.
+        2:{ apply lc_tlete_tapp_tm_assoc_source. exact Hlc. }
+        2:{ set_solver. }
+        rewrite formula_open_expr_result_formula_shift0.
+        2:{ apply lc_tapp_tm; [exact Hlc | constructor]. }
+        2:{ set_solver. }
+        pose proof (res_models_fuel_scoped _ _ _ Hopen) as Hscope_src.
+        match goal with
+        | |- my ⊨ ?G =>
+            assert (Hscope_tgt_outer : formula_scoped_in_world my G)
+        end.
+        {
+          unfold formula_scoped_in_world in *.
+          normalize_denotation_formula_fv_in Hscope_src.
+          normalize_formula_fv.
+          try rewrite fv_tm_tapp_tm_tlete_assoc.
+          exact Hscope_src.
+        }
+        eapply res_models_impl_intro; [exact Hscope_tgt_outer|].
+        intros Hbasic.
+        match goal with
+        | |- my ⊨ ?G =>
+            assert (Hscope_tgt_inner : formula_scoped_in_world my G)
+        end.
+        { eapply formula_scoped_impl_r. exact Hscope_tgt_outer. }
+        eapply res_models_impl_intro; [exact Hscope_tgt_inner|].
+        intros Hresult.
+        pose proof (res_models_impl_elim _ _ _ Hopen Hbasic) as Hinner.
+        eapply res_models_impl_elim; [exact Hinner|].
+        eapply expr_result_formula_tapp_tm_tlete_assoc_rev.
+        -- rewrite fv_tm_tapp_tm_tlete_assoc.
+           eapply denot_ty_lvar_guard_wfworld_closed_on_term_le.
+           ++ eapply res_extend_by_le; exact Hext.
+           ++ repeat rewrite res_models_and_iff. exact Hguard.
+        -- exact Hlc.
+        -- exact Hresult.
+      * exact Hbody.
+    + solve_tapp_tlete_guard_assoc.
+    + repeat rewrite res_models_and_iff in Hbody |- *.
+      destruct Hbody as [H1 H2].
+      split; [eapply IH | eapply IH]; eauto.
+    + solve_tapp_tlete_guard_assoc.
+    + pose proof (res_models_fuel_scoped _ _ _ Hbody) as Hscope.
+      eapply res_models_or_transport_between_worlds
+        with (m := m) (φa := denot_ty_lvar_gas gas Σ τ1
+          (tlete e1 (tapp_tm e2 (vfvar y))))
+          (φb := denot_ty_lvar_gas gas Σ τ2
+          (tlete e1 (tapp_tm e2 (vfvar y)))).
+      * pose proof (denot_ty_lvar_gas_scope_from_relevant_guard
+          (S gas) Σ (CTUnion τ1 τ2)
+          (tapp_tm (tlete e1 e2) (vfvar y)) m
+          ltac:(repeat rewrite res_models_and_iff;
+            solve_tapp_tlete_guard_assoc)) as Hscope_full.
+        cbn [denot_ty_lvar_gas] in Hscope_full.
+        eapply formula_scoped_or_l.
+        eapply formula_scoped_and_r. exact Hscope_full.
+      * pose proof (denot_ty_lvar_gas_scope_from_relevant_guard
+          (S gas) Σ (CTUnion τ1 τ2)
+          (tapp_tm (tlete e1 e2) (vfvar y)) m
+          ltac:(repeat rewrite res_models_and_iff;
+            solve_tapp_tlete_guard_assoc)) as Hscope_full.
+        cbn [denot_ty_lvar_gas] in Hscope_full.
+        eapply formula_scoped_or_r.
+        eapply formula_scoped_and_r. exact Hscope_full.
+      * intros Hτ1. eapply IH; eauto.
+      * intros Hτ2. eapply IH; eauto.
+      * exact Hbody.
+    + solve_tapp_tlete_guard_assoc.
+    + pose proof (res_models_fuel_scoped _ _ _ Hbody) as Hscope.
+      apply res_models_plus_iff in Hbody as
+        [m1 [m2 [Hdef [Hle [H1 H2]]]]].
+      * eapply res_models_plus_intro_from_models; [exact Hle| |].
+        -- eapply IH; eauto.
+        -- eapply IH; eauto.
+      * exact Hscope.
+    + solve_tapp_tlete_guard_assoc.
+    + lazymatch type of Hbody with
+      | m ⊨ FForall ?φsrc => eapply (res_models_forall_full_world_map m φsrc)
+      end.
+      * pose proof (denot_ty_lvar_gas_scope_from_relevant_guard
+          (S gas) Σ (CTArrow τx τr)
+          (tapp_tm (tlete e1 e2) (vfvar y)) m
+          ltac:(repeat rewrite res_models_and_iff;
+            solve_tapp_tlete_guard_assoc)) as Hscope_full.
+        cbn [denot_ty_lvar_gas] in Hscope_full.
+        eapply formula_scoped_and_r; exact Hscope_full.
+      * exists (fv_tm (tapp_tm (tlete e1 e2) (vfvar y)) ∪
+          fv_tm (tlete e1 (tapp_tm e2 (vfvar y))) ∪
+          fv_cty τx ∪ fv_cty τr ∪ lvars_fv (dom Σ)).
+        intros z Hz my Hdom Hrestrict Hopen.
+        pose proof (denot_ty_lvar_gas_scope_from_relevant_guard
+          (S gas) Σ (CTArrow τx τr)
+          (tapp_tm (tlete e1 e2) (vfvar y)) m
+          ltac:(repeat rewrite res_models_and_iff;
+            solve_tapp_tlete_guard_assoc)) as Hscope_full_my.
+        cbn [denot_ty_lvar_gas] in Hscope_full_my.
+        pose proof (formula_scoped_and_r _ _ _ Hscope_full_my)
+          as Htarget_forall_scope.
+        match goal with
+        | |- my ⊨ ?G =>
+            assert (Hopened_scope_my : formula_scoped_in_world my G)
+        end.
+        {
+          eapply formula_scoped_open_from_fv.
+          unfold formula_scoped_in_world in Htarget_forall_scope.
+          rewrite Hdom.
+          set_solver.
+        }
+        repeat rewrite formula_open_impl in Hopen.
+        repeat rewrite formula_open_impl.
+        repeat rewrite formula_open_impl in Hopened_scope_my.
+        rewrite ?formula_open_basic_world_bind0 in Hopen |- *
+          by tlet_support_solver.
+        rewrite ?formula_open_basic_world_bind0 in Hopened_scope_my
+          by tlet_support_solver.
+        eapply res_models_impl_intro; [exact Hopened_scope_my|].
+        intros Hbasic.
+        pose proof (formula_scoped_impl_r _ _ _ Hopened_scope_my)
+          as Hscope_tgt_inner.
+        eapply res_models_impl_intro; [exact Hscope_tgt_inner|].
+        intros Harg.
+        assert (Henv_arrow :
+          denot_relevant_env Σ (CTArrow τx τr)
+            (tapp_tm (tlete e1 e2) (vfvar y)) =
+          denot_relevant_env Σ (CTArrow τx τr)
+            (tlete e1 (tapp_tm e2 (vfvar y)))).
+        {
+          unfold denot_relevant_env, denot_relevant_lvars,
+            lty_env_restrict_lvars.
+          rewrite tm_lvars_tapp_tm_tlete_assoc_fvar. reflexivity.
+        }
+        rewrite Henv_arrow in Harg.
+        pose proof (res_models_impl_elim _ _ _ Hopen Hbasic) as Hinner.
+        pose proof (res_models_impl_elim _ _ _ Hinner Harg) as Hres.
+        pose proof (res_models_open_denot_ty_lvar_gas_to_open
+          z gas
+          (denot_relevant_env Σ (CTArrow τx τr)
+            (tlete e1 (tapp_tm e2 (vfvar y))))
+          (erase_ty τx) τr
+          (tapp_tm (tm_shift 0 (tlete e1 (tapp_tm e2 (vfvar y)))) (vbvar 0))
+          my
+          ltac:(unfold denot_relevant_env, lty_env_restrict_lvars;
+            change (LVFree z ∉ dom (storeA_restrict (Σ : gmap logic_var ty)
+              (denot_relevant_lvars (CTArrow τx τr)
+                (tlete e1 (tapp_tm e2 (vfvar y))))));
+            rewrite storeA_restrict_dom;
+            intros Hzdom; apply elem_of_intersection in Hzdom as [HzΣ _];
+            apply Hz; repeat (apply elem_of_union_r);
+            apply lvars_fv_elem; exact HzΣ)
+          ltac:(apply denot_relevant_env_closed; exact HΣ)
+          ltac:(rewrite fv_tapp_tm, tm_shift_fv; cbn [fv_value]; set_solver)
+          ltac:(set_solver)
+          Hres) as Hres_opened.
+        clear Hres. rename Hres_opened into Hres.
+        cbn [open_tm open_value value_shift] in Hres.
+        rewrite open_tapp_tm_shift_bvar0_lc in Hres
+          by (apply lc_tlete_tapp_tm_assoc_source; exact Hlc).
+        eapply denot_ty_lvar_gas_tapp_tlete_assoc_under_tapp in Hres.
+        3:{ exact Hlc. }
+        2:{
+          apply lty_env_closed_insert_free.
+          apply denot_relevant_env_closed. exact HΣ.
+        }
+        rewrite <- Henv_arrow in Hres.
+        replace (tapp_tm (tapp_tm (tlete e1 e2) (vfvar y)) (vfvar z))
+          with (open_tm 0 (vfvar z)
+            (tapp_tm (tm_shift 0 (tapp_tm (tlete e1 e2) (vfvar y))) (vbvar 0)))
+          in Hres by
+          (rewrite open_tapp_tm_shift_bvar0_lc by
+            (apply lc_tapp_tm; [exact Hlc | constructor]);
+           reflexivity).
+        pose proof (res_models_open_denot_ty_lvar_gas_from_open
+          z gas
+          (denot_relevant_env Σ (CTArrow τx τr)
+            (tapp_tm (tlete e1 e2) (vfvar y)))
+          (erase_ty τx) τr
+          (tapp_tm (tm_shift 0 (tapp_tm (tlete e1 e2) (vfvar y))) (vbvar 0))
+          my
+          ltac:(unfold denot_relevant_env, lty_env_restrict_lvars;
+            change (LVFree z ∉ dom (storeA_restrict (Σ : gmap logic_var ty)
+              (denot_relevant_lvars (CTArrow τx τr)
+                (tapp_tm (tlete e1 e2) (vfvar y)))));
+            rewrite storeA_restrict_dom;
+            intros Hzdom; apply elem_of_intersection in Hzdom as [HzΣ _];
+            apply Hz; repeat (apply elem_of_union_r);
+            apply lvars_fv_elem; exact HzΣ)
+          ltac:(apply denot_relevant_env_closed; exact HΣ)
+          ltac:(rewrite fv_tapp_tm, tm_shift_fv; cbn [fv_value]; set_solver)
+          ltac:(set_solver)
+          Hres) as Hres_formula.
+        clear Hres. rename Hres_formula into Hres.
+        exact Hres.
+      * exact Hbody.
+    + solve_tapp_tlete_guard_assoc.
+    + lazymatch type of Hbody with
+      | m ⊨ FForall ?φsrc => eapply (res_models_forall_full_world_map m φsrc)
+      end.
+      * pose proof (denot_ty_lvar_gas_scope_from_relevant_guard
+          (S gas) Σ (CTWand τx τr)
+          (tapp_tm (tlete e1 e2) (vfvar y)) m
+          ltac:(repeat rewrite res_models_and_iff;
+            solve_tapp_tlete_guard_assoc)) as Hscope_full.
+        cbn [denot_ty_lvar_gas] in Hscope_full.
+        eapply formula_scoped_and_r; exact Hscope_full.
+      * exists (fv_tm (tapp_tm (tlete e1 e2) (vfvar y)) ∪
+          fv_tm (tlete e1 (tapp_tm e2 (vfvar y))) ∪
+          fv_cty τx ∪ fv_cty τr ∪ lvars_fv (dom Σ)).
+        intros z Hz my Hdom Hrestrict Hopen.
+        repeat rewrite formula_open_impl in Hopen.
+        repeat rewrite formula_open_impl.
+        rewrite ?formula_open_basic_world_bind0 in Hopen |- *
+          by tlet_support_solver.
+        rewrite !formula_open_wand in Hopen |- *.
+        pose proof (denot_ty_lvar_gas_scope_from_relevant_guard
+          (S gas) Σ (CTWand τx τr)
+          (tapp_tm (tlete e1 e2) (vfvar y)) m
+          ltac:(repeat rewrite res_models_and_iff;
+            solve_tapp_tlete_guard_assoc)) as Hscope_full_my.
+        cbn [denot_ty_lvar_gas] in Hscope_full_my.
+        pose proof (formula_scoped_and_r _ _ _ Hscope_full_my)
+          as Htarget_forall_scope.
+        match goal with
+        | |- my ⊨ ?G =>
+            assert (Hscope_tgt_outer : formula_scoped_in_world my G)
+        end.
+        {
+          change (formula_scoped_in_world my
+            (formula_open 0 z
+              (FImpl (basic_world_formula (<[LVBound 0 := erase_ty τx]> ∅))
+                (FWand
+                  (denot_ty_lvar_gas gas
+                    (typed_lty_env_bind
+                      (denot_relevant_env Σ (CTWand τx τr)
+                        (tapp_tm (tlete e1 e2) (vfvar y)))
+                      (erase_ty τx))
+                    (cty_shift 0 τx) (tret (vbvar 0)))
+                  (denot_ty_lvar_gas gas
+                    (typed_lty_env_bind
+                      (denot_relevant_env Σ (CTWand τx τr)
+                        (tapp_tm (tlete e1 e2) (vfvar y)))
+                      (erase_ty τx))
+                    τr
+                    (tapp_tm
+                      (tm_shift 0 (tapp_tm (tlete e1 e2) (vfvar y)))
+                      (vbvar 0))))))).
+          eapply formula_scoped_open_from_fv.
+          unfold formula_scoped_in_world in Htarget_forall_scope.
+          formula_fv_syntax_norm_in Htarget_forall_scope.
+          formula_fv_syntax_norm.
+          rewrite Hdom.
+          set_solver.
+        }
+        eapply res_models_impl_intro; [exact Hscope_tgt_outer|].
+        intros Hbasic.
+        pose proof (res_models_impl_elim _ _ _ Hopen Hbasic) as Hwand.
+        pose proof (res_models_fuel_scoped _ _ _ Hwand) as Hscope_src_wand.
+        pose proof (proj1 (res_models_wand_iff my _ _ Hscope_src_wand) Hwand)
+          as Hwand_elim.
+        clear Hwand. rename Hwand_elim into Hwand.
+        pose proof (formula_scoped_impl_r _ _ _ Hscope_tgt_outer)
+             as Hscope_tgt_wand.
+        apply (proj2 (res_models_wand_iff _ _ _ Hscope_tgt_wand)).
+        intros n1 Hc Harg.
+              assert (Henv_wand :
+                denot_relevant_env Σ (CTWand τx τr)
+                  (tapp_tm (tlete e1 e2) (vfvar y)) =
+                denot_relevant_env Σ (CTWand τx τr)
+                  (tlete e1 (tapp_tm e2 (vfvar y)))).
+              {
+                unfold denot_relevant_env, denot_relevant_lvars,
+                  lty_env_restrict_lvars.
+                rewrite tm_lvars_tapp_tm_tlete_assoc_fvar. reflexivity.
+	              }
+	              rewrite Henv_wand in Harg.
+	              pose proof (Hwand n1 Hc Harg) as Hres.
+	              pose proof (res_models_open_denot_ty_lvar_gas_to_open
+	                z gas
+	                (denot_relevant_env Σ (CTWand τx τr)
+	                  (tlete e1 (tapp_tm e2 (vfvar y))))
+	                (erase_ty τx) τr
+	                (tapp_tm (tm_shift 0 (tlete e1 (tapp_tm e2 (vfvar y)))) (vbvar 0))
+	                (res_product n1 my Hc)
+	                ltac:(unfold denot_relevant_env, lty_env_restrict_lvars;
+	                  change (LVFree z ∉ dom (storeA_restrict (Σ : gmap logic_var ty)
+	                    (denot_relevant_lvars (CTWand τx τr)
+	                      (tlete e1 (tapp_tm e2 (vfvar y))))));
+	                  rewrite storeA_restrict_dom;
+	                  intros Hzdom; apply elem_of_intersection in Hzdom as [HzΣ _];
+	                  apply Hz; repeat (apply elem_of_union_r);
+	                  apply lvars_fv_elem; exact HzΣ)
+	                ltac:(apply denot_relevant_env_closed; exact HΣ)
+	                ltac:(rewrite fv_tapp_tm, tm_shift_fv; cbn [fv_value]; set_solver)
+	                ltac:(set_solver)
+	                Hres) as Hres_opened.
+	              clear Hres. rename Hres_opened into Hres.
+	              cbn [open_tm open_value value_shift] in Hres.
+	              rewrite open_tapp_tm_shift_bvar0_lc in Hres
+	                by (apply lc_tlete_tapp_tm_assoc_source; exact Hlc).
+	              eapply denot_ty_lvar_gas_tapp_tlete_assoc_under_tapp in Hres.
+	              3:{ exact Hlc. }
+	              2:{
+	                apply lty_env_closed_insert_free.
+	                apply denot_relevant_env_closed. exact HΣ.
+	              }
+	              rewrite <- Henv_wand in Hres.
+	              replace (tapp_tm (tapp_tm (tlete e1 e2) (vfvar y)) (vfvar z))
+	                with (open_tm 0 (vfvar z)
+	                  (tapp_tm (tm_shift 0 (tapp_tm (tlete e1 e2) (vfvar y))) (vbvar 0)))
+	                in Hres by
+	                (rewrite open_tapp_tm_shift_bvar0_lc by
+	                  (apply lc_tapp_tm; [exact Hlc | constructor]);
+	                 reflexivity).
+	              pose proof (res_models_open_denot_ty_lvar_gas_from_open
+	                z gas
+	                (denot_relevant_env Σ (CTWand τx τr)
+	                  (tapp_tm (tlete e1 e2) (vfvar y)))
+	                (erase_ty τx) τr
+	                (tapp_tm (tm_shift 0 (tapp_tm (tlete e1 e2) (vfvar y))) (vbvar 0))
+	                (res_product n1 my Hc)
+	                ltac:(unfold denot_relevant_env, lty_env_restrict_lvars;
+	                  change (LVFree z ∉ dom (storeA_restrict (Σ : gmap logic_var ty)
+	                    (denot_relevant_lvars (CTWand τx τr)
+	                      (tapp_tm (tlete e1 e2) (vfvar y)))));
+	                  rewrite storeA_restrict_dom;
+	                  intros Hzdom; apply elem_of_intersection in Hzdom as [HzΣ _];
+	                  apply Hz; repeat (apply elem_of_union_r);
+	                  apply lvars_fv_elem; exact HzΣ)
+	                ltac:(apply denot_relevant_env_closed; exact HΣ)
+	                ltac:(rewrite fv_tapp_tm, tm_shift_fv; cbn [fv_value]; set_solver)
+	                ltac:(set_solver)
+	                Hres) as Hres_formula.
+	              clear Hres. rename Hres_formula into Hres.
+	              exact Hres.
+      * exact Hbody.
+Qed.
+Lemma tlet_wand_open_body_transport
+    gas (Σ : lty_env) (T1 : ty) (e1 e2 : tm)
+    (m mx my myx : WfWorldT) (Fx : FiberExtensionT)
+    (x y : atom) τx τr :
+  (forall (Σ : lty_env) (T1 : ty) (e1 e2 : tm)
+     (m mx : WfWorldT) (Fx : FiberExtensionT) (x : atom)
+     (τ : context_ty),
+    lty_env_closed Σ ->
+    lty_env_to_atom_env Σ ⊢ₑ e1 ⋮ T1 ->
+    lty_env_to_atom_env Σ ⊢ₑ tlete e1 e2 ⋮ erase_ty τ ->
+    expr_result_extension_witness e1 x Fx ->
+    m ⊨ expr_total_formula e1 ->
+    m ⊨ basic_world_formula (denot_relevant_env Σ τ (tlete e1 e2)) ->
+    LVFree x ∉ dom Σ ∪ context_ty_lvars τ ->
+    res_extend_by m Fx mx ->
+    mx ⊨ denot_ty_lvar_gas gas (<[LVFree x := T1]> Σ) τ (e2 ^^ x) ->
+    m ⊨ denot_ty_lvar_gas gas Σ τ (tlete e1 e2)) ->
+  lty_env_closed Σ ->
+  lty_env_to_atom_env Σ ⊢ₑ e1 ⋮ T1 ->
+  lty_env_to_atom_env Σ ⊢ₑ tlete e1 e2 ⋮ erase_ty (CTWand τx τr) ->
+  expr_result_extension_witness e1 x Fx ->
+  m ⊨ expr_total_formula e1 ->
+  m ⊨ basic_world_formula
+    (denot_relevant_env Σ (CTWand τx τr) (tlete e1 e2)) ->
+  LVFree x ∉ dom Σ ∪ context_ty_lvars (CTWand τx τr) ->
+  y ∉ lvars_fv (dom Σ) ∪ fv_tm e1 ∪ fv_tm e2 ∪
+    fv_cty τx ∪ fv_cty τr ∪ {[x]} ->
+  x <> y ->
+  y ∉ fv_cty τx ->
+  y ∉ fv_cty τr ->
+  LVFree y ∉ dom
+    (denot_relevant_env Σ (CTWand τx τr) (tlete e1 e2) : lty_env) ->
+  LVFree y ∉ dom
+    (denot_relevant_env (<[LVFree x := T1]> Σ)
+      (CTWand τx τr) (e2 ^^ x) : lty_env) ->
+  LVFree y ∉ dom (<[LVFree x := T1]> Σ : lty_env) ->
+  lc_tm (e2 ^^ x) ->
+  y ∉ fv_tm (tapp_tm (tm_shift 0 (e2 ^^ x)) (vbvar 0)) ->
+  basic_context_ty_lvars
+    (dom (<[LVFree x := T1]> Σ : lty_env) : gset logic_var)
+    (CTWand τx τr) ->
+  m ⊑ my ->
+  world_dom (my : WorldT) = world_dom (m : WorldT) ∪ {[y]} ->
+  res_extend_by my Fx myx ->
+  formula_scoped_in_world my
+    (formula_open 0 y
+      (denot_wand_body_formula gas
+        (denot_relevant_env Σ (CTWand τx τr) (tlete e1 e2))
+        τx τr (tlete e1 e2))) ->
+  myx ⊨ formula_open 0 y
+    (denot_wand_body_formula gas
+      (denot_relevant_env (<[LVFree x := T1]> Σ)
+        (CTWand τx τr) (e2 ^^ x))
+      τx τr (e2 ^^ x)) ->
+  my ⊨ formula_open 0 y
+    (denot_wand_body_formula gas
+      (denot_relevant_env Σ (CTWand τx τr) (tlete e1 e2))
+      τx τr (tlete e1 e2)).
+Proof.
+  intros IH HΣ He1 Hlet HFx Htotal Hbase_world Hfresh
+    Hy_support Hxy Hyτx Hyτr Hy_target_rel Hy_source_rel Hy_insert
+    Hlc_e2x Hy_body_fv Hbasic_src_rel
+    Hle Hdom_my HmyFx Hscope_target Hbody.
+  unfold denot_wand_body_formula in Hscope_target, Hbody |- *.
+  rewrite formula_open_impl in Hbody |- *.
+  rewrite formula_open_wand in Hbody |- *.
+  rewrite ?formula_open_basic_world_bind0 in Hbody |- * by tlet_support_solver.
+  eapply res_models_impl_intro; [exact Hscope_target|].
+  intros Hbasic.
+  pose proof (res_models_impl_elim _ _ _ Hbody
+    ltac:(eapply res_models_extend_mono; [exact HmyFx | exact Hbasic]))
+    as Hsource_wand.
+  pose proof (formula_scoped_impl_r _ _ _ Hscope_target) as Hscope_target_wand.
+  eapply res_models_wand_intro; [exact Hscope_target_wand|].
+  intros n Hc Harg.
+  assert (Hxτx : LVFree x ∉ context_ty_lvars τx).
+  {
+    cbn [context_ty_lvars context_ty_lvars_at] in Hfresh.
+    fast_set_solver!!.
+  }
+  set (source_arg :=
+    formula_open 0 y
+      (denot_ty_lvar_gas gas
+        (typed_lty_env_bind
+          (denot_relevant_env (<[LVFree x := T1]> Σ)
+            (CTWand τx τr) (e2 ^^ x))
+          (erase_ty τx))
+        (cty_shift 0 τx) (tret (vbvar 0)))).
+  set (source_body :=
+    formula_open 0 y
+      (denot_ty_lvar_gas gas
+        (typed_lty_env_bind
+          (denot_relevant_env (<[LVFree x := T1]> Σ)
+            (CTWand τx τr) (e2 ^^ x))
+          (erase_ty τx))
+        τr
+        (tapp_tm (tm_shift 0 (e2 ^^ x)) (vbvar 0)))).
+  change (myx ⊨ FWand source_arg source_body) in Hsource_wand.
+  pose proof (tlet_wand_arg_source_from_target
+    gas Σ T1 x y τx τr e1 e2 n
+    HΣ Hxy Hxτx
+    Hyτx Hy_target_rel Hy_source_rel Harg) as Harg_source_n.
+  change (n ⊨ source_arg) in Harg_source_n.
+  set (n0 := res_restrict n (formula_fv source_arg)).
+  assert (Harg_source_n0 : n0 ⊨ source_arg).
+  { subst n0. apply res_models_restrict_fv. exact Harg_source_n. }
+  assert (Hout_source_arg : extA_out Fx ## formula_fv source_arg).
+  {
+    pose proof (proj2 (expr_result_extension_witness_shape _ _ _ HFx))
+      as HoutFx.
+    unfold ext_out in HoutFx.
+    pose proof (tlet_wand_source_arg_fresh_x
+      gas Σ T1 x y τx τr e1 e2 HΣ Hxy Hxτx) as Hxfv.
+    rewrite HoutFx. set_solver.
+  }
+  assert (Hc0_my : world_compat n0 my).
+  { subst n0. eapply world_compat_le_l; [apply res_restrict_le | exact Hc]. }
+  assert (Hc0_myx : world_compat n0 myx).
+  {
+    eapply world_compat_restrict_l_extend_by_fresh;
+      [exact Hout_source_arg | exact HmyFx | exact Hc].
+  }
+  pose proof (res_models_wand_elim n0 myx Hc0_myx
+    source_arg source_body Hsource_wand Harg_source_n0)
+    as Hsource_body_prod.
+  assert (Hsource_body_for_ih :
+    res_product n0 myx Hc0_myx ⊨ denot_ty_lvar_gas gas
+      (<[LVFree x := T1]> (<[LVFree y := erase_ty τx]> Σ))
+      (cty_open 0 y τr)
+      ((tapp_tm e2 (vfvar y)) ^^ x)).
+	  {
+	    subst source_body.
+	    eapply tlet_wand_source_body_open_for_ih.
+	    - exact HΣ.
+	    - exact Hxy.
+	    - cbn [context_ty_lvars context_ty_lvars_at] in Hfresh |- *.
+	      fast_set_solver!!.
+	    - exact Hy_source_rel.
+	    - exact Hy_insert.
+	    - exact Hlc_e2x.
+	    - exact Hy_body_fv.
+	    - exact Hyτr.
+	    - exact Hbasic_src_rel.
+	    - exact Hsource_body_prod.
+	  }
+  assert (Hout_n0_dom : extA_out Fx ## world_dom (n0 : WorldT)).
+  {
+	    subst n0.
+	    pose proof (proj2 (expr_result_extension_witness_shape _ _ _ HFx))
+	      as HoutFx.
+	    unfold ext_out in HoutFx.
+	    unfold world_dom, res_restrict. simpl.
+	    rewrite HoutFx in Hout_source_arg.
+	    set_solver.
+	  }
+  pose proof (res_extend_by_product_r_fresh n0 my myx Fx
+    Hc0_my Hc0_myx Hout_n0_dom HmyFx) as Hprod_ext.
+  assert (Hbasic_src_rel0 :
+    basic_context_ty_lvars (dom (Σ : gmap logic_var ty) : gset logic_var)
+      (CTWand τx τr)).
+  {
+    destruct Hbasic_src_rel as [Hvars Hshape]. split; [|exact Hshape].
+    intros v Hv.
+    specialize (Hvars v Hv).
+    change (v ∈ dom ((<[LVFree x := T1]> (Σ : gmap logic_var ty))
+      : gmap logic_var ty)) in Hvars.
+    rewrite dom_insert_L in Hvars.
+    apply elem_of_union in Hvars as [Hvx|HvΣ]; [|exact HvΣ].
+    apply elem_of_singleton in Hvx. subst v.
+    exfalso. apply Hfresh. apply elem_of_union_r. exact Hv.
+  }
+  assert (HlcΣ : lc_lvars (dom (Σ : gmap logic_var ty) : gset logic_var)).
+  { apply (proj2 (lc_lvars_no_bv _)). exact HΣ. }
+  assert (HyΣ : LVFree y ∉ (dom (Σ : gmap logic_var ty) : gset logic_var)).
+  {
+    intros HyΣ.
+    assert (Hyfv : y ∈ lvars_fv (dom (Σ : gmap logic_var ty) : gset logic_var)).
+    { apply lvars_fv_elem. exact HyΣ. }
+    apply Hy_support.
+    fast_set_solver!!.
+  }
+  assert (Hclosed_Σy : lty_env_closed (<[LVFree y := erase_ty τx]> Σ)).
+  { apply lty_env_closed_insert_free. exact HΣ. }
+  assert (He1_Σy :
+    lty_env_to_atom_env (<[LVFree y := erase_ty τx]> Σ) ⊢ₑ e1 ⋮ T1).
+  {
+    eapply basic_typing_env_agree_tm; [exact He1|].
+    intros a Ha.
+    rewrite !lty_env_to_atom_env_lookup.
+    change (((<[LVFree y := erase_ty τx]> (Σ : gmap logic_var ty))
+      : gmap logic_var ty) !! LVFree a =
+      (Σ : gmap logic_var ty) !! LVFree a).
+    rewrite lookup_insert_ne; [reflexivity|].
+    intros Hbad. inversion Hbad. subst a.
+    apply Hy_support. fast_set_solver!!.
+  }
+  assert (Hlet_Σy :
+    lty_env_to_atom_env (<[LVFree y := erase_ty τx]> Σ) ⊢ₑ
+      tlete e1 (tapp_tm e2 (vfvar y)) ⋮ erase_ty (cty_open 0 y τr)).
+  {
+    rewrite cty_open_preserves_erasure.
+    apply basic_typing_tapp_tm_tlete_assoc_rev.
+    eapply basic_typing_tapp_tm.
+    - eapply basic_typing_env_agree_tm; [exact Hlet|].
+      intros a Ha.
+      rewrite !lty_env_to_atom_env_lookup.
+      change (((<[LVFree y := erase_ty τx]> (Σ : gmap logic_var ty))
+        : gmap logic_var ty) !! LVFree a =
+        (Σ : gmap logic_var ty) !! LVFree a).
+      rewrite lookup_insert_ne; [reflexivity|].
+      intros Hbad. inversion Hbad. subst a.
+      apply Hy_support. fast_set_solver!!.
+    - constructor.
+      rewrite lty_env_to_atom_env_lookup.
+      change (((<[LVFree y := erase_ty τx]> (Σ : gmap logic_var ty))
+        : gmap logic_var ty) !! LVFree y = Some (erase_ty τx)).
+      rewrite lookup_insert.
+      destruct (decide (LVFree y = LVFree y)); [reflexivity|congruence].
+  }
+  assert (Htotal_prod :
+    res_product n0 my Hc0_my ⊨ expr_total_formula e1).
+  {
+    eapply res_models_kripke.
+    - etransitivity.
+      + exact Hle.
+      + apply res_product_le_r_tlet.
+    - exact Htotal.
+  }
+  assert (Hbase_world_prod :
+    res_product n0 my Hc0_my ⊨ basic_world_formula
+      (denot_relevant_env (<[LVFree y := erase_ty τx]> Σ)
+        (cty_open 0 y τr) (tlete e1 (tapp_tm e2 (vfvar y))))).
+  {
+    eapply basic_world_formula_wand_body_from_source_and_arg.
+    - exact HlcΣ.
+    - exact HyΣ.
+    - exact Hbasic_src_rel0.
+    - apply tm_lvars_tlet_tapp_tm_fvar_without_arg.
+    - eapply res_models_kripke.
+      + apply res_product_le_r_tlet.
+      + eapply res_models_kripke; [exact Hle|exact Hbase_world].
+    - eapply res_models_kripke.
+      + apply res_product_le_r_tlet.
+      + rewrite formula_open_basic_world_formula in Hbasic.
+        rewrite lty_env_open_one_bound0_singleton in Hbasic.
+        exact Hbasic.
+  }
+  assert (Hfresh_x_Σy :
+    LVFree x ∉ dom (<[LVFree y := erase_ty τx]> Σ) ∪
+      context_ty_lvars (cty_open 0 y τr)).
+  {
+    intros Hbad.
+    apply elem_of_union in Hbad as [Hdom|Hτ].
+    - change (LVFree x ∈ dom ((<[LVFree y := erase_ty τx]>
+        (Σ : gmap logic_var ty)) : gmap logic_var ty)) in Hdom.
+      rewrite dom_insert_L in Hdom.
+      apply elem_of_union in Hdom as [Hyx|HxΣ].
+      + apply elem_of_singleton in Hyx. inversion Hyx. congruence.
+      + cbn [context_ty_lvars context_ty_lvars_at] in Hfresh.
+        fast_set_solver!!.
+    - assert (Hdiff :
+        LVFree x ∈ context_ty_lvars (cty_open 0 y τr) ∖ {[LVFree y]}).
+      { set_solver. }
+      pose proof (context_ty_lvars_open_body_without_fresh_closed
+        (dom (Σ : gmap logic_var ty) : gset logic_var) τr y
+        HlcΣ HyΣ ltac:(destruct Hbasic_src_rel0 as [Hvars _];
+          cbn [context_ty_lvars context_ty_lvars_at] in Hvars |- *;
+          set_solver)) as Hsubset.
+      specialize (Hsubset _ Hdiff).
+      cbn [context_ty_lvars context_ty_lvars_at] in Hfresh.
+      fast_set_solver!!.
+  }
+  pose proof (IH (<[LVFree y := erase_ty τx]> Σ) T1 e1
+    (tapp_tm e2 (vfvar y))
+    (res_product n0 my Hc0_my) (res_product n0 myx Hc0_myx)
+    Fx x (cty_open 0 y τr)
+    Hclosed_Σy He1_Σy Hlet_Σy HFx Htotal_prod Hbase_world_prod
+    Hfresh_x_Σy Hprod_ext Hsource_body_for_ih) as HIH_result.
+  assert (Htarget_body_small :
+    res_product n0 my Hc0_my ⊨ formula_open 0 y
+      (denot_ty_lvar_gas gas
+        (typed_lty_env_bind
+          (denot_relevant_env Σ (CTWand τx τr) (tlete e1 e2))
+          (erase_ty τx))
+        τr
+        (tapp_tm (tm_shift 0 (tlete e1 e2)) (vbvar 0)))).
+  {
+    assert (Hassoc :
+      res_product n0 my Hc0_my ⊨ denot_ty_lvar_gas gas
+        (<[LVFree y := erase_ty τx]> Σ)
+        (cty_open 0 y τr)
+        (tapp_tm (tlete e1 e2) (vfvar y))).
+    {
+      eapply denot_ty_lvar_gas_tapp_tlete_assoc.
+      - exact Hclosed_Σy.
+      - eapply typing_tm_lc. exact Hlet.
+      - exact HIH_result.
+    }
+    pose proof (res_models_denot_ty_lvar_gas_env_agree_on
+      gas (<[LVFree y := erase_ty τx]> Σ)
+      (<[LVFree y := erase_ty τx]>
+        (denot_relevant_env Σ (CTWand τx τr) (tlete e1 e2)))
+      (cty_open 0 y τr) (tapp_tm (tlete e1 e2) (vfvar y))
+      (denot_relevant_lvars (cty_open 0 y τr)
+        (tapp_tm (tlete e1 e2) (vfvar y)))
+      (res_product n0 my Hc0_my)
+      ltac:(intros v Hv; exact Hv)
+      ltac:(symmetry;
+        eapply wand_body_relevant_env_agree_from_basic_context_ty;
+        [exact HlcΣ|exact HyΣ|exact Hbasic_src_rel0|
+         apply tm_lvars_tapp_tm_fvar_without_arg])
+      Hassoc) as Henv.
+    replace (tapp_tm (tlete e1 e2) (vfvar y)) with
+      (open_tm 0 (vfvar y)
+        (tapp_tm (tm_shift 0 (tlete e1 e2)) (vbvar 0))) in Henv.
+    2:{
+      rewrite open_tapp_tm_shift_bvar0_lc.
+      - reflexivity.
+      - eapply typing_tm_lc. exact Hlet.
+    }
+    eapply res_models_open_denot_ty_lvar_gas_from_open.
+    - exact Hy_target_rel.
+    - apply denot_relevant_env_closed. exact HΣ.
+    - rewrite fv_tapp_tm, tm_shift_fv. cbn [fv_value].
+      fast_set_solver!!.
+    - exact Hyτr.
+    - exact Henv.
+  }
+  eapply res_models_kripke.
+  - eapply res_product_le_mono.
+    + apply res_restrict_le.
+    + reflexivity.
+  - exact Htarget_body_small.
+Qed.
+
+
+
+Lemma tlet_intro_denotation_wand_case
+    gas (Σ : lty_env) (T1 : ty) (e1 e2 : tm)
+    (m mx : WfWorldT) (Fx : FiberExtensionT) (x : atom)
+    τx τr :
+  (forall (Σ : lty_env) (T1 : ty) (e1 e2 : tm)
+     (m mx : WfWorldT) (Fx : FiberExtensionT) (x : atom)
+     (τ : context_ty),
+    lty_env_closed Σ ->
+    lty_env_to_atom_env Σ ⊢ₑ e1 ⋮ T1 ->
+    lty_env_to_atom_env Σ ⊢ₑ tlete e1 e2 ⋮ erase_ty τ ->
+    expr_result_extension_witness e1 x Fx ->
+    m ⊨ expr_total_formula e1 ->
+    m ⊨ basic_world_formula (denot_relevant_env Σ τ (tlete e1 e2)) ->
+    LVFree x ∉ dom Σ ∪ context_ty_lvars τ ->
+    res_extend_by m Fx mx ->
+    mx ⊨ denot_ty_lvar_gas gas (<[LVFree x := T1]> Σ) τ (e2 ^^ x) ->
+    m ⊨ denot_ty_lvar_gas gas Σ τ (tlete e1 e2)) ->
+  lty_env_closed Σ ->
+  lty_env_to_atom_env Σ ⊢ₑ e1 ⋮ T1 ->
+  lty_env_to_atom_env Σ ⊢ₑ tlete e1 e2 ⋮ erase_ty (CTWand τx τr) ->
+  expr_result_extension_witness e1 x Fx ->
+  m ⊨ expr_total_formula e1 ->
+  m ⊨ basic_world_formula
+    (denot_relevant_env Σ (CTWand τx τr) (tlete e1 e2)) ->
+  LVFree x ∉ dom Σ ∪ context_ty_lvars (CTWand τx τr) ->
+  res_extend_by m Fx mx ->
+  mx ⊨ denot_ty_lvar_gas (S gas)
+    (<[LVFree x := T1]> Σ) (CTWand τx τr) (e2 ^^ x) ->
+  m ⊨ denot_ty_lvar_gas (S gas) Σ (CTWand τx τr) (tlete e1 e2).
+Proof.
+  intros IH HΣ He1 Hlet HFx Htotal Hbase_world Hfresh Hext Hmx.
+  cbn [denot_ty_lvar_gas] in Hmx |- *.
+  normalize_models_ands_in Hmx; normalize_models_ands_goal.
+  destruct Hmx as [Hmx_guard Hmx_wand_body].
+  assert (HxΣ : LVFree x ∉ dom Σ) by tlet_support_solver.
+  assert (Hxτ : LVFree x ∉ context_ty_lvars (CTWand τx τr))
+    by tlet_support_solver.
+  assert (Hmx_zero : mx ⊨ denot_ty_lvar_gas 0
+    (<[LVFree x := T1]> Σ) (CTWand τx τr) (e2 ^^ x)).
+  {
+    cbn [denot_ty_lvar_gas].
+    rewrite res_models_and_iff. split.
+    - repeat rewrite res_models_and_iff. exact Hmx_guard.
+    - cbn [res_models res_models_fuel formula_measure].
+      split; [apply formula_scoped_true_iff; exact I | exact I].
+  }
+  pose proof (tlet_intro_denotation_gas_zero_support
+    Σ T1 e1 e2 m mx Fx x (CTWand τx τr)
+    HΣ He1 Hlet HFx Htotal Hbase_world HxΣ Hxτ Hext Hmx_zero)
+    as Hm_zero.
+  assert (Hguard_m :
+    m ⊨ FAnd
+      (context_ty_wf_formula
+        (denot_relevant_env Σ (CTWand τx τr) (tlete e1 e2))
+        (CTWand τx τr))
+      (FAnd
+        (basic_world_formula
+          (denot_relevant_env Σ (CTWand τx τr) (tlete e1 e2)))
+        (FAnd
+          (expr_basic_typing_formula
+            (denot_relevant_env Σ (CTWand τx τr) (tlete e1 e2))
+            (tlete e1 e2) (erase_ty (CTWand τx τr)))
+          (expr_total_formula (tlete e1 e2))))).
+  {
+    cbn [denot_ty_lvar_gas] in Hm_zero.
+    rewrite res_models_and_iff in Hm_zero.
+    exact (proj1 Hm_zero).
+  }
+  assert (Hdenot_scope_m :
+    formula_scoped_in_world m
+      (denot_ty_lvar_gas (S gas) Σ (CTWand τx τr) (tlete e1 e2))).
+  {
+    eapply denot_ty_lvar_gas_scope_from_relevant_guard.
+    exact Hguard_m.
+  }
+  assert (Hbody_scope_m :
+    formula_scoped_in_world m
+      (FForall
+        (FImpl
+          (basic_world_formula (<[LVBound 0 := erase_ty τx]> ∅))
+          (FWand
+            (denot_ty_lvar_gas gas
+              (typed_lty_env_bind
+                (denot_relevant_env Σ (CTWand τx τr) (tlete e1 e2))
+                (erase_ty τx))
+              (cty_shift 0 τx) (tret (vbvar 0)))
+            (denot_ty_lvar_gas gas
+              (typed_lty_env_bind
+                (denot_relevant_env Σ (CTWand τx τr) (tlete e1 e2))
+                (erase_ty τx))
+              τr
+              (tapp_tm (tm_shift 0 (tlete e1 e2)) (vbvar 0))))))).
+  {
+    cbn [denot_ty_lvar_gas] in Hdenot_scope_m.
+    eapply formula_scoped_and_r. exact Hdenot_scope_m.
+  }
+  split.
+  - repeat rewrite res_models_and_iff in Hguard_m.
+    exact Hguard_m.
+	- refine (res_models_forall_ext_transport
+	    m mx Fx _ _ Hbody_scope_m Hext _ Hmx_wand_body).
+	  exists (lvars_fv (dom Σ) ∪ fv_tm e1 ∪ fv_tm e2 ∪
+	    fv_cty τx ∪ fv_cty τr ∪ {[x]}).
+	  intros y Hy my myx Hle Hdom_my HmyFx Hmyx_body.
+	  assert (Htarget_open_scope :
+	    formula_scoped_in_world my
+	      (formula_open 0 y
+	        (denot_wand_body_formula gas
+	          (denot_relevant_env Σ (CTWand τx τr) (tlete e1 e2))
+	          τx τr (tlete e1 e2)))).
+	  {
+	    unfold denot_wand_body_formula.
+	    pose proof (formula_scoped_forall_body m _ Hbody_scope_m)
+	      as Hforall_body_scope_m.
+	    assert (Hy_my : y ∈ world_dom (my : WorldT)).
+	    { rewrite Hdom_my. set_solver. }
+	    eapply formula_scoped_open_res_le;
+	      [exact Hforall_body_scope_m | exact Hle | exact Hy_my].
+	  }
+	  assert (Hxy : x <> y).
+	  { intros ->. apply Hy. fast_set_solver!!. }
+	  assert (Hxτx : LVFree x ∉ context_ty_lvars τx).
+	  {
+	    cbn [context_ty_lvars context_ty_lvars_at] in Hfresh.
+	    fast_set_solver!!.
+	  }
+	  assert (Hyτx : y ∉ fv_cty τx) by fast_set_solver!!.
+	  assert (Hyτr : y ∉ fv_cty τr) by fast_set_solver!!.
+	  assert (Hy_target_rel : LVFree y ∉ dom
+	    (denot_relevant_env Σ (CTWand τx τr) (tlete e1 e2) : lty_env)).
+	  {
+	    intros HyD. apply Hy.
+	    assert (Hyfv : y ∈ lvars_fv (dom
+	      (denot_relevant_env Σ (CTWand τx τr) (tlete e1 e2) : lty_env))).
+	    { apply lvars_fv_elem. exact HyD. }
+	    pose proof (denot_relevant_env_fv_subset
+	      Σ (CTWand τx τr) (tlete e1 e2)) as Hrel.
+	    pose proof (Hrel y Hyfv) as Hyrel.
+	    unfold fv_cty, context_ty_lvars in *.
+	    cbn [fv_cty context_ty_lvars context_ty_lvars_at fv_tm] in Hyrel.
+	    try rewrite lvars_fv_union in Hyrel.
+	    try rewrite !context_ty_lvars_fv_at in Hyrel.
+	    clear - Hy Hyrel. set_solver.
+	  }
+	  assert (Hy_source_rel : LVFree y ∉ dom
+	    (denot_relevant_env (<[LVFree x := T1]> Σ)
+	      (CTWand τx τr) (e2 ^^ x) : lty_env)).
+	  {
+	    intros HyD. apply Hy.
+	    assert (Hyfv : y ∈ lvars_fv (dom
+	      (denot_relevant_env (<[LVFree x := T1]> Σ)
+	        (CTWand τx τr) (e2 ^^ x) : lty_env))).
+	    { apply lvars_fv_elem. exact HyD. }
+	    pose proof (denot_relevant_env_fv_subset
+	      (<[LVFree x := T1]> Σ) (CTWand τx τr) (e2 ^^ x)) as Hrel.
+	    pose proof (Hrel y Hyfv) as Hyrel.
+	    pose proof (open_fv_tm e2 (vfvar x) 0 y) as Hopen.
+	    unfold fv_cty, context_ty_lvars in *.
+	    cbn [fv_cty context_ty_lvars context_ty_lvars_at fv_value] in Hyrel, Hopen.
+	    try rewrite lvars_fv_union in Hyrel.
+	    try rewrite !context_ty_lvars_fv_at in Hyrel.
+	    clear - Hy Hyrel Hopen. set_solver.
+	  }
+	  assert (Hy_insert : LVFree y ∉ dom (<[LVFree x := T1]> Σ : lty_env)).
+	  {
+	    change (LVFree y ∉ dom
+	      ((<[LVFree x := T1]> (Σ : gmap logic_var ty)) : gmap logic_var ty)).
+	    rewrite dom_insert_L.
+	    intros Hybad. apply Hy.
+		    apply elem_of_union in Hybad as [Hyx | HyΣ].
+		    - apply elem_of_singleton in Hyx. inversion Hyx. congruence.
+		    - assert (HyΣfv : y ∈ lvars_fv (dom (Σ : gmap logic_var ty))).
+		      { rewrite lvars_fv_elem. exact HyΣ. }
+		      set_solver.
+		  }
+	  assert (Hlc_e2x : lc_tm (e2 ^^ x)).
+	  { eapply tlet_lc_open_body_from_basic; exact Hlet. }
+	  assert (Hy_body_fv :
+	    y ∉ fv_tm (tapp_tm (tm_shift 0 (e2 ^^ x)) (vbvar 0))).
+	  {
+	    rewrite fv_tapp_tm, tm_shift_fv.
+	    cbn [fv_value].
+	    intros Hybad.
+	    apply elem_of_union in Hybad as [Hye2x | Hyempty].
+	    - pose proof (open_fv_tm e2 (vfvar x) 0 y Hye2x) as Hcases.
+	      cbn [fv_value] in Hcases.
+	      apply Hy. fast_set_solver!!.
+	    - set_solver.
+	  }
+	  assert (Hbasic_src_rel :
+	    basic_context_ty_lvars
+	      (dom (<[LVFree x := T1]> Σ : lty_env) : gset logic_var)
+	      (CTWand τx τr)).
+	  {
+	    pose proof Hmx_guard as Hmx_guard_parts.
+	    repeat rewrite res_models_and_iff in Hmx_guard_parts.
+	    destruct Hmx_guard_parts as [Hmx_wf _].
+	    pose proof (context_ty_wf_formula_basic_lvars _ _ _ Hmx_wf)
+	      as Hbasic_rel.
+	    eapply basic_context_ty_lvars_mono; [|exact Hbasic_rel].
+	    apply denot_relevant_env_dom_subset_direct.
+	  }
+	  eapply tlet_wand_open_body_transport; eauto.
+Qed.
+
+Ltac open_formula_syntax_step :=
+  rewrite ?formula_open_impl;
+  rewrite ?formula_open_fibvars;
+  rewrite ?formula_open_over;
+  rewrite ?formula_open_under;
+  rewrite ?formula_open_context_ty_wf_formula;
+  rewrite ?formula_open_expr_total_formula by solve_tlet_sidecond;
+  rewrite ?formula_open_basic_world_bind0 by solve_tlet_sidecond;
+  rewrite ?formula_open_basic_world_formula;
+  rewrite ?formula_open_expr_result_formula_shift0 by solve_tlet_sidecond;
+  rewrite ?formula_open_expr_result_formula by solve_tlet_sidecond;
+  rewrite ?lvars_open_qual_vars_difference_bound0;
+  rewrite ?type_qualifier_formula_open by solve_tlet_sidecond;
+  rewrite ?open_tapp_tm_fvar_lc_arg.
+
+Ltac normalize_open_denot_goal :=
+  idtac;
+  rewrite ?open_tapp_tm_fvar_lc_arg.
 
 Ltac normalize_open_denot_in H :=
   transport_open_denot_in H;
